some wrong admits about alloc,free in final erasure. Should have used a different relation.

concurrency/SC_erasure.v
@@ -36,51 +36,61 @@ Set Bullet Behavior "Strict Subproofs".
 (** ** Erasure of Values*)
 Module ValErasure.
 
-  Definition erased_val v1 v2 : Prop :=
+  Definition val_erasure v1 v2 : Prop :=
     match v1, v2 with
     | Vundef, _ => True
     | v1, v2 => v1 = v2
     end.
 
-  Definition erased_memval mv1 mv2 : Prop :=
+  Definition memval_erasure mv1 mv2 : Prop :=
     match mv1, mv2 with
     | Undef, _ => True
+    | Fragment v1 q1 n1, Fragment v2 q2 n2 =>
+      val_erasure v1 v2 /\ q1 = q2 /\ n1 = n2
     | mv1, mv2 => mv1 = mv2
     end.
   
-  Inductive erased_val_list : seq.seq val -> seq.seq val -> Prop :=
-    erased_val_nil : erased_val_list [::] [::]
-  | erased_val_cons : forall (v v' : val) (vl vl' : seq.seq val),
-      erased_val v v' ->
-      erased_val_list vl vl' ->
-      erased_val_list (v :: vl) (v' :: vl').
+  Inductive val_erasure_list : seq.seq val -> seq.seq val -> Prop :=
+    val_erasure_nil : val_erasure_list [::] [::]
+  | val_erasure_cons : forall (v v' : val) (vl vl' : seq.seq val),
+      val_erasure v v' ->
+      val_erasure_list vl vl' ->
+      val_erasure_list (v :: vl) (v' :: vl').
 
-  Inductive erased_memval_list : seq.seq memval -> seq.seq memval -> Prop :=
-    erased_memval_nil : erased_memval_list [::] [::]
-  | erased_memval_cons : forall (mv mv' : memval) (mvl mvl' : seq.seq memval),
-      erased_memval mv mv' ->
-      erased_memval_list mvl mvl' ->
-      erased_memval_list (mv :: mvl) (mv' :: mvl').
+  Inductive memval_erasure_list : seq.seq memval -> seq.seq memval -> Prop :=
+    memval_erasure_nil : memval_erasure_list [::] [::]
+  | memval_erasure_cons : forall (mv mv' : memval) (mvl mvl' : seq.seq memval),
+      memval_erasure mv mv' ->
+      memval_erasure_list mvl mvl' ->
+      memval_erasure_list (mv :: mvl) (mv' :: mvl').
 
-  Lemma erased_val_refl:
-    forall v, erased_val v v.
+  Lemma val_erasure_refl:
+    forall v, val_erasure v v.
   Proof.
     destruct v; simpl; auto.
   Qed.
 
-  Hint Immediate erased_val_refl : erased.
-  Hint Constructors erased_val_list : erased.
+  Lemma memval_erasure_refl:
+    forall mval,
+      memval_erasure mval mval.
+  Proof.
+    intros; destruct mval; constructor;
+    eauto using val_erasure_refl.
+  Qed.
+
+  Hint Immediate memval_erasure_refl val_erasure_refl : val_erasure.
+  Hint Constructors memval_erasure_list val_erasure_list : val_erasure.
   
-  Lemma erased_val_list_refl:
-    forall vs, erased_val_list vs vs.
-  Proof with eauto with erased.
+  Lemma val_erasure_list_refl:
+    forall vs, val_erasure_list vs vs.
+  Proof with eauto with val_erasure.
     induction vs; simpl...
   Qed.
 
-  Lemma erased_val_list_decode:
+  Lemma val_erasure_list_decode:
     forall vals vals' typs,
-      erased_val_list vals vals' ->
-      erased_val_list (decode_longs typs vals) (decode_longs typs vals').
+      val_erasure_list vals vals' ->
+      val_erasure_list (decode_longs typs vals) (decode_longs typs vals').
   Proof.
     intros.
     generalize dependent vals.
@@ -96,44 +106,685 @@ Module ValErasure.
     destruct v;
       constructor; eauto;
       inv H2; try constructor.
-    unfold erased_val in H3.
+    unfold val_erasure in H3.
     destruct v0; subst; auto;
     constructor.
   Qed.
 
+  Lemma memval_erasure_list_refl:
+    forall vs, memval_erasure_list vs vs.
+  Proof with eauto with val_erasure.
+    induction vs; simpl...
+  Qed.
+
+  Hint Immediate memval_erasure_list_refl : val_erasure.
+
   (** ** Lemmas about erased values*)
-  Lemma erased_val_hiword:
+
+  Definition isPointer (v : val) :=
+    match v with
+    | Vptr _ _ => true
+    | _ => false
+    end.
+
+  Definition isDefined v :=
+    match v with
+    | Vundef => false
+    | _ => true
+    end.
+  
+  Lemma val_erasure_add_result:
+    forall v1 v1' v2 v2' v,
+      val_erasure v1 v1' ->
+      val_erasure v2 v2' ->
+      Val.add v1 v2 = v ->
+      isDefined v ->
+      Val.add v1' v2' = v.
+  Proof.
+    intros.
+    destruct v1,v2; simpl in *; subst; simpl in *;
+    try (by exfalso); auto.
+  Qed.
+
+  Lemma isPointer_isDefined:
+    forall v, isPointer v -> isDefined v.
+  Proof.
+    unfold isPointer, isDefined;
+    destruct v; auto.
+  Qed.
+  
+  Lemma val_erasure_add:
+    forall v1 v2 v1' v2',
+      val_erasure v1 v1' ->
+      val_erasure v2 v2' ->
+      val_erasure (Val.add v1 v2) (Val.add v1' v2').
+  Proof.
+    destruct v1,v2; intros;
+    simpl; auto;
+    inv H; inv H0; simpl; auto.
+  Qed.
+
+  Lemma val_erasure_mul:
+    forall v1 v2 v1' v2',
+      val_erasure v1 v1' ->
+      val_erasure v2 v2' ->
+      val_erasure (Val.mul v1 v2) (Val.mul v1' v2').
+  Proof.
+    destruct v1,v2; intros;
+    simpl; auto;
+    inv H; inv H0; simpl; auto.
+  Qed.
+  
+  Lemma val_erasure_mul_result:
+    forall v1 v2 v1' v2' v,
+      val_erasure v1 v1'->
+      val_erasure v2 v2' ->
+      Val.mul v1 v2 = v ->
+      isDefined v ->
+      Val.mul v1' v2' = v.
+  Proof.
+    intros.
+    destruct v1,v2; simpl in *; subst; simpl in *;
+    try by exfalso.
+    reflexivity.
+  Qed.
+  
+  Lemma val_erasure_hiword:
     forall v v',
-      erased_val v v' ->
-      erased_val (Val.hiword v) (Val.hiword v').
+      val_erasure v v' ->
+      val_erasure (Val.hiword v) (Val.hiword v').
   Proof.
     intros;
     destruct v; simpl; inv H; auto.
   Qed.
 
-  Lemma erased_val_loword:
+  Lemma val_erasure_loword:
     forall v v',
-      erased_val v v' ->
-      erased_val (Val.loword v) (Val.loword v').
+      val_erasure v v' ->
+      val_erasure (Val.loword v) (Val.loword v').
   Proof.
     intros;
     destruct v; simpl; inv H; auto.
   Qed.
 
-  Lemma erased_val_cmp_bool:
+  Lemma val_erasure_cmp_bool:
     forall c v1 v1',
       v1 <> Vundef ->
-      erased_val v1 v1' ->
+      val_erasure v1 v1' ->
       Val.cmp_bool c v1 Vzero = Val.cmp_bool c v1' Vzero.
   Proof.
     intros.
     destruct v1; try congruence.
   Qed.
 
-  Hint Resolve erased_val_hiword erased_val_loword : erased.
+  Lemma val_erasure_zero_ext:
+    forall v v' n,
+      val_erasure v v' ->
+      val_erasure (Val.zero_ext n v) (Val.zero_ext n v').
+  Proof.
+    intros.
+    destruct v; inv H; simpl; auto.
+  Qed.
+
+  Lemma val_erasure_sign_ext:
+    forall v v' n,
+      val_erasure v v' ->
+      val_erasure (Val.sign_ext n v) (Val.sign_ext n v').
+  Proof.
+    intros.
+    destruct v; inv H; simpl; auto.
+  Qed.
+
+  Lemma val_erasure_singleoffloat:
+    forall v v',
+      val_erasure v v' ->
+      val_erasure (Val.singleoffloat v) (Val.singleoffloat v').
+  Proof.
+    intros.
+    destruct v; inv H; simpl; auto.
+  Qed.
+
+  Lemma val_erasure_floatofsingle:
+    forall v v',
+      val_erasure v v' ->
+      val_erasure (Val.floatofsingle v) (Val.floatofsingle v').
+  Proof.
+    intros.
+    destruct v; inv H; simpl; auto.
+  Qed.
+
+  Lemma val_erasure_intoffloat:
+    forall v v',
+      val_erasure v v' ->
+      val_erasure (Val.maketotal (Val.intoffloat v))
+                  (Val.maketotal (Val.intoffloat v')).
+  Proof.
+    intros.
+    destruct v; inv H; simpl; eauto using val_erasure_refl.
+  Qed.
+
+  Lemma val_erasure_floatofint:
+    forall v v',
+      val_erasure v v' ->
+      val_erasure (Val.maketotal (Val.floatofint v))
+                  (Val.maketotal (Val.floatofint v')).
+  Proof.
+    intros.
+    destruct v; inv H; simpl; eauto using val_erasure_refl.
+  Qed.
+
+  Lemma val_erasure_intofsingle:
+    forall v v',
+      val_erasure v v' ->
+      val_erasure (Val.maketotal (Val.intofsingle v))
+                  (Val.maketotal (Val.intofsingle v')).
+  Proof.
+    intros.
+    destruct v; inv H; simpl; eauto using val_erasure_refl.
+  Qed.
+  
+  Lemma val_erasure_singleofint:
+    forall v v',
+      val_erasure v v' ->
+      val_erasure (Val.maketotal (Val.singleofint v))
+                  (Val.maketotal (Val.singleofint v')).
+  Proof.
+    intros.
+    destruct v; inv H; simpl; eauto using val_erasure_refl.
+  Qed.
+
+  
+  Lemma val_erasure_neg:
+    forall v v',
+      val_erasure v v' ->
+      val_erasure (Val.neg v) (Val.neg v').
+  Proof.
+    intros.
+    destruct v; inv H; simpl; auto.
+  Qed.
+
+  Lemma val_erasure_notint:
+    forall v v',
+      val_erasure v v' ->
+      val_erasure (Val.notint v) (Val.notint v').
+  Proof.
+    intros.
+    destruct v; inv H; simpl; auto.
+  Qed.
+
+  Lemma val_erasure_negative:
+    forall v v',
+      val_erasure v v' ->
+      val_erasure (Val.negative v) (Val.negative v').
+  Proof.
+    intros.
+    destruct v; inv H; simpl; auto.
+  Qed.
+
+  Lemma val_erasure_sub_overflow:
+    forall v1 v2 v1' v2',
+      val_erasure v1 v1' ->
+      val_erasure v2 v2' ->
+      val_erasure (Val.sub_overflow v1 v2) (Val.sub_overflow v1' v2').
+  Proof.
+    destruct v1,v2; intros;
+    simpl; auto;
+    inv H; inv H0; simpl; auto.
+  Qed.
+  
+  Lemma val_erasure_sub:
+    forall v1 v2 v1' v2',
+      val_erasure v1 v1' ->
+      val_erasure v2 v2' ->
+      val_erasure (Val.sub v1 v2) (Val.sub v1' v2').
+  Proof.
+    destruct v1,v2; intros;
+    simpl; auto;
+    inv H; inv H0; simpl; auto.
+    destruct (eq_block b b0); simpl; auto.
+  Qed.
+
+  Lemma val_erasure_mulhu:
+    forall v1 v2 v1' v2',
+      val_erasure v1 v1' ->
+      val_erasure v2 v2' ->
+      val_erasure (Val.mulhu v1 v2) (Val.mulhu v1' v2').
+  Proof.
+    destruct v1,v2; intros;
+    simpl; auto;
+    inv H; inv H0; simpl; auto.
+  Qed.
+
+  Lemma val_erasure_mulhs:
+    forall v1 v2 v1' v2',
+      val_erasure v1 v1' ->
+      val_erasure v2 v2' ->
+      val_erasure (Val.mulhs v1 v2) (Val.mulhs v1' v2').
+  Proof.
+    destruct v1,v2; intros;
+    simpl; auto;
+    inv H; inv H0; simpl; auto.
+  Qed.
+
+  Lemma val_erasure_and:
+    forall v1 v2 v1' v2',
+      val_erasure v1 v1' ->
+      val_erasure v2 v2' ->
+      val_erasure (Val.and v1 v2) (Val.and v1' v2').
+  Proof.
+    destruct v1,v2; intros;
+    simpl; auto;
+    inv H; inv H0; simpl; auto.
+  Qed.
+
+  Lemma val_erasure_or:
+    forall v1 v2 v1' v2',
+      val_erasure v1 v1' ->
+      val_erasure v2 v2' ->
+      val_erasure (Val.or v1 v2) (Val.or v1' v2').
+  Proof.
+    destruct v1,v2; intros;
+    simpl; auto;
+    inv H; inv H0; simpl; auto.
+  Qed.
+
+  Lemma val_erasure_xor:
+    forall v1 v2 v1' v2',
+      val_erasure v1 v1' ->
+      val_erasure v2 v2' ->
+      val_erasure (Val.xor v1 v2) (Val.xor v1' v2').
+  Proof.
+    destruct v1,v2; intros;
+    simpl; auto;
+    inv H; inv H0; simpl; auto.
+  Qed.
+
+  Lemma val_erasure_shl:
+    forall v1 v2 v1' v2',
+      val_erasure v1 v1' ->
+      val_erasure v2 v2' ->
+      val_erasure (Val.shl v1 v2) (Val.shl v1' v2').
+  Proof.
+    destruct v1,v2; intros;
+    simpl; auto;
+    inv H; inv H0; simpl; eauto using val_erasure_refl.
+  Qed.
+
+  Lemma val_erasure_shr:
+    forall v1 v2 v1' v2',
+      val_erasure v1 v1' ->
+      val_erasure v2 v2' ->
+      val_erasure (Val.shr v1 v2) (Val.shr v1' v2').
+  Proof.
+    destruct v1,v2; intros;
+    simpl; auto;
+    inv H; inv H0; simpl; eauto using val_erasure_refl.
+  Qed.
+
+  Lemma val_erasure_shru:
+    forall v1 v2 v1' v2',
+      val_erasure v1 v1' ->
+      val_erasure v2 v2' ->
+      val_erasure (Val.shru v1 v2) (Val.shru v1' v2').
+  Proof.
+    destruct v1,v2; intros;
+    simpl; auto;
+    inv H; inv H0; simpl; eauto using val_erasure_refl.
+  Qed.
+
+  Lemma val_erasure_ror:
+    forall v1 v2 v1' v2',
+      val_erasure v1 v1' ->
+      val_erasure v2 v2' ->
+      val_erasure (Val.ror v1 v2) (Val.ror v1' v2').
+  Proof.
+    destruct v1,v2; intros;
+    simpl; auto;
+    inv H; inv H0; simpl; eauto using val_erasure_refl.
+  Qed.
+
+  Lemma val_erasure_divu_result:
+    forall v1 v2 v1' v2' v,
+      val_erasure v1 v1' ->
+      val_erasure v2 v2' ->
+      Val.divu v1 v2 = Some v ->
+      Val.divu v1' v2' = Some v.
+  Proof.
+    destruct v1,v2; intros;
+    inv H; inv H0; simpl in *; eauto using val_erasure_refl;
+    try discriminate.
+  Qed.
+
+  Lemma val_erasure_modu_result:
+    forall v1 v2 v1' v2' v,
+      val_erasure v1 v1' ->
+      val_erasure v2 v2' ->
+      Val.modu v1 v2 = Some v ->
+      Val.modu v1' v2' = Some v.
+  Proof.
+    destruct v1,v2; intros;
+    inv H; inv H0; simpl in *; eauto using val_erasure_refl;
+    try discriminate.
+  Qed.
+
+  Lemma val_erasure_divs_result:
+    forall v1 v2 v1' v2' v,
+      val_erasure v1 v1' ->
+      val_erasure v2 v2' ->
+      Val.divs v1 v2 = Some v ->
+      Val.divs v1' v2' = Some v.
+  Proof.
+    destruct v1,v2; intros;
+    inv H; inv H0; simpl in *; eauto using val_erasure_refl;
+    try discriminate.
+  Qed.
+
+  Lemma val_erasure_mods_result:
+    forall v1 v2 v1' v2' v,
+      val_erasure v1 v1' ->
+      val_erasure v2 v2' ->
+      Val.mods v1 v2 = Some v ->
+      Val.mods v1' v2' = Some v.
+  Proof.
+    destruct v1,v2; intros;
+    inv H; inv H0; simpl in *; eauto using val_erasure_refl;
+    try discriminate.
+  Qed.
+
+  Lemma val_erasure_addf:
+    forall v1 v2 v1' v2',
+      val_erasure v1 v1' ->
+      val_erasure v2 v2' ->
+      val_erasure (Val.addf v1 v2) (Val.addf v1' v2').
+  Proof.
+    destruct v1,v2; intros;
+    simpl; auto;
+    inv H; inv H0; simpl; auto.
+  Qed.
+
+  Lemma val_erasure_addfs:
+    forall v1 v2 v1' v2',
+      val_erasure v1 v1' ->
+      val_erasure v2 v2' ->
+      val_erasure (Val.addfs v1 v2) (Val.addfs v1' v2').
+  Proof.
+    destruct v1,v2; intros;
+    simpl; auto;
+    inv H; inv H0; simpl; auto.
+  Qed.
+  
+  Lemma val_erasure_subf:
+    forall v1 v2 v1' v2',
+      val_erasure v1 v1' ->
+      val_erasure v2 v2' ->
+      val_erasure (Val.subf v1 v2) (Val.subf v1' v2').
+  Proof.
+    destruct v1,v2; intros;
+    simpl; auto;
+    inv H; inv H0; simpl; auto.
+  Qed.
+
+  Lemma val_erasure_subfs:
+    forall v1 v2 v1' v2',
+      val_erasure v1 v1' ->
+      val_erasure v2 v2' ->
+      val_erasure (Val.subfs v1 v2) (Val.subfs v1' v2').
+  Proof.
+    destruct v1,v2; intros;
+    simpl; auto;
+    inv H; inv H0; simpl; auto.
+  Qed.
+
+  Lemma val_erasure_mulf:
+    forall v1 v2 v1' v2',
+      val_erasure v1 v1' ->
+      val_erasure v2 v2' ->
+      val_erasure (Val.mulf v1 v2) (Val.mulf v1' v2').
+  Proof.
+    destruct v1,v2; intros;
+    simpl; auto;
+    inv H; inv H0; simpl; auto.
+  Qed.
+
+  Lemma val_erasure_mulfs:
+    forall v1 v2 v1' v2',
+      val_erasure v1 v1' ->
+      val_erasure v2 v2' ->
+      val_erasure (Val.mulfs v1 v2) (Val.mulfs v1' v2').
+  Proof.
+    destruct v1,v2; intros;
+    simpl; auto;
+    inv H; inv H0; simpl; auto.
+  Qed.
+
+  Lemma val_erasure_divf:
+    forall v1 v2 v1' v2',
+      val_erasure v1 v1' ->
+      val_erasure v2 v2' ->
+      val_erasure (Val.divf v1 v2) (Val.divf v1' v2').
+  Proof.
+    destruct v1,v2; intros;
+    simpl; auto;
+    inv H; inv H0; simpl; auto.
+  Qed.
+
+  Lemma val_erasure_divfs:
+    forall v1 v2 v1' v2',
+      val_erasure v1 v1' ->
+      val_erasure v2 v2' ->
+      val_erasure (Val.divfs v1 v2) (Val.divfs v1' v2').
+  Proof.
+    destruct v1,v2; intros;
+    simpl; auto;
+    inv H; inv H0; simpl; auto.
+  Qed.
+
+  Lemma val_erasure_negf:
+    forall v v',
+      val_erasure v v' ->
+      val_erasure (Val.negf v) (Val.negf v').
+  Proof.
+    intros.
+    destruct v; inv H; simpl; auto.
+  Qed.
+
+  Lemma val_erasure_negfs:
+    forall v v',
+      val_erasure v v' ->
+      val_erasure (Val.negfs v) (Val.negfs v').
+  Proof.
+    intros.
+    destruct v; inv H; simpl; auto.
+  Qed.
+  
+  Lemma val_erasure_absf:
+    forall v v',
+      val_erasure v v' ->
+      val_erasure (Val.absf v) (Val.absf v').
+  Proof.
+    intros.
+    destruct v; inv H; simpl; auto.
+  Qed.
+
+  Lemma val_erasure_absfs:
+    forall v v',
+      val_erasure v v' ->
+      val_erasure (Val.absfs v) (Val.absfs v').
+  Proof.
+    intros.
+    destruct v; inv H; simpl; auto.
+  Qed.
+
+  Lemma inj_bytes_erasure :
+    forall (bl : seq.seq byte),
+      memval_erasure_list (inj_bytes bl) (inj_bytes bl).
+  Proof.
+    induction bl;
+    simpl; constructor; auto.
+    constructor.
+  Qed.
+
+  Lemma inj_value_erasure :
+    forall (v1 v2 : val) (q : quantity),
+      val_erasure v1 v2 ->
+      memval_erasure_list (inj_value q v1) (inj_value q v2).
+  Proof with eauto with val_erasure.
+    intros.
+    destruct v1; inv H; simpl...
+    destruct q; simpl; unfold inj_value; simpl;
+    repeat (econstructor; simpl; auto).
+  Qed.
+    
+  Lemma repeat_Undef_erasure_self :
+    forall (n : nat),
+      memval_erasure_list (list_repeat n Undef) (list_repeat n Undef).
+  Proof.
+    eauto with val_erasure.
+  Qed.
+
+  Lemma repeat_Undef_inject_encode_val :
+    forall (chunk : memory_chunk) (v : val),
+      memval_erasure_list (list_repeat (size_chunk_nat chunk) Undef)
+                         (encode_val chunk v).
+  Proof with eauto with val_erasure.
+    intros.
+    destruct v, chunk; simpl; unfold inj_value; simpl;
+    repeat econstructor...
+  Qed.
+    
+  Lemma val_erasure_encode_val:
+    forall chunk v v',
+      val_erasure v v' ->
+      memval_erasure_list (encode_val chunk v) (encode_val chunk v').
+  Proof.
+    intros. 
+    destruct v; inversion H; subst; simpl; destruct chunk;
+    auto using inj_bytes_erasure,  inj_value_erasure, repeat_Undef_erasure_self,
+    repeat_Undef_inject_encode_val.    
+    unfold encode_val. destruct v'; apply inj_value_erasure; auto.
+    unfold encode_val. destruct v'; apply inj_value_erasure; auto.
+  Qed.
+  
+  Lemma val_defined_add_1:
+    forall v1 v2 v,
+      Val.add v1 v2 = v ->
+      isDefined v ->
+      isDefined v1.
+  Proof.
+    intros. destruct v1,v2; subst; simpl; auto.
+  Qed.
+
+  Lemma val_defined_add_2:
+    forall v1 v2 v,
+      Val.add v1 v2 = v ->
+      isDefined v ->
+      isDefined v2.
+  Proof.
+    intros. destruct v1,v2; subst; simpl; auto.
+  Qed.
+
+  Hint Resolve val_defined_add_1 val_defined_add_2 : val_defined.
+
+  Hint Extern 0 (val_erasure (Vint _) (Vint _)) => reflexivity : val_erasure.
+  Hint Resolve val_erasure_ror val_erasure_shru val_erasure_shr
+       val_erasure_shl val_erasure_xor val_erasure_or val_erasure_and
+       val_erasure_mulhs val_erasure_mulhu val_erasure_sub
+       val_erasure_neg val_erasure_singleofint val_erasure_singleoffloat
+       val_erasure_intofsingle val_erasure_floatofint val_erasure_intoffloat
+       val_erasure_floatofsingle val_erasure_singleoffloat val_erasure_sign_ext
+       val_erasure_zero_ext val_erasure_negative val_erasure_notint
+       val_erasure_sub_overflow val_erasure_encode_val
+       val_erasure_hiword val_erasure_loword
+       val_erasure_add val_erasure_add_result isPointer_isDefined
+       val_erasure_mul_result val_erasure_mul
+       val_erasure_addf val_erasure_subf val_erasure_mulf
+       val_erasure_divf val_erasure_negf val_erasure_absf
+       val_erasure_addfs val_erasure_subfs val_erasure_mulfs
+       val_erasure_divfs val_erasure_negfs val_erasure_absfs : val_erasure.
+
+  Hint Immediate val_erasure_refl : val_erasure.
 
 End ValErasure.
 
+(** ** Erasure of Traces*)
+Module TraceErasure.
+  Import ValErasure event_semantics.
+
+  Inductive mem_event_erasure : mem_event -> mem_event -> Prop :=
+  | WriteErasure: forall b ofs mvals mvals',
+      memval_erasure_list mvals mvals' ->
+      mem_event_erasure (Write b ofs mvals) (Write b ofs mvals')
+  | ReadErasure: forall b ofs sz mvals mvals',
+      memval_erasure_list mvals mvals' ->
+      mem_event_erasure (Read b ofs sz mvals) (Read b ofs sz mvals')
+  | AllocErasure: forall b ofs sz,
+      mem_event_erasure (Alloc b ofs sz) (Alloc b ofs sz)
+  | FreeErasure: forall ls,
+      mem_event_erasure (Free ls) (Free ls).
+
+  Inductive mem_event_list_erasure: list mem_event -> list mem_event -> Prop :=
+  | nilMemEvent: mem_event_list_erasure nil nil
+  | consMemEvent: forall mev mev' ls ls'
+                   (Hev_erasure: mem_event_erasure mev mev')
+                   (Hls_erasure: mem_event_list_erasure ls ls'),
+      mem_event_list_erasure (mev :: ls) (mev' :: ls').
+  
+  Inductive event_erasure : Events.machine_event -> Events.machine_event -> Prop :=
+  | InternalErasure: forall tid mev mev',
+      mem_event_erasure mev mev' ->
+      event_erasure (Events.internal tid mev) (Events.internal tid mev')
+  | ExternalErasure: forall tid ev,
+      event_erasure (Events.external tid ev) (Events.external tid ev).
+
+  Inductive trace_erasure : list Events.machine_event ->
+                            list Events.machine_event -> Prop :=
+  | NilErasure: trace_erasure nil nil
+  | ConsErasure: forall ev ev' tr tr'
+                   (Hev_erasure: event_erasure ev ev')
+                   (Htr_erasure: trace_erasure tr tr'),
+      trace_erasure (ev :: tr) (ev' :: tr').
+
+  Lemma mem_event_list_erasure_cat:
+    forall tr1 tr1' tr2 tr2',
+      mem_event_list_erasure tr1 tr1' ->
+      mem_event_list_erasure tr2 tr2' ->
+      mem_event_list_erasure (tr1 ++ tr2) (tr1' ++ tr2').
+  Proof.
+    induction tr1 as [|ev tr1]; intros; inv H.
+    simpl; auto.
+    simpl.
+    constructor; eauto.
+  Qed.
+        
+  Lemma trace_erasure_cat:
+    forall tr1 tr1' tr2 tr2',
+      trace_erasure tr1 tr1' ->
+      trace_erasure tr2 tr2' ->
+      trace_erasure (tr1 ++ tr2) (tr1' ++ tr2').
+  Proof.
+    induction tr1 as [|ev tr1]; intros; inv H.
+    simpl; auto.
+    simpl.
+    constructor; eauto.
+  Qed.
+
+  Lemma trace_erasure_map:
+    forall ev ev' tid,
+      mem_event_list_erasure ev ev' ->
+      trace_erasure (map [eta Events.internal tid] ev)
+                    (map [eta Events.internal tid] ev').
+  Proof.
+    induction 1;
+    simpl; constructor; auto.
+    constructor; auto.
+  Qed.
+
+
+  Hint Resolve trace_erasure_cat trace_erasure_map : trace_erasure.
+  Hint Constructors trace_erasure event_erasure : trace_erasure.
+
+End TraceErasure.
+    
 (** ** Memory Erasure*)
 Module MemErasure.
 
@@ -144,31 +795,31 @@ Module MemErasure.
 
   Local Notation "a # b" := (PMap.get b a) (at level 1).
 
-  Record erasedMem (m m': mem) :=
+  Record mem_erasure (m m': mem) :=
     { perm_le:
         forall b ofs k,
           Mem.valid_block m' b -> 
           (Mem.mem_access m')#b ofs k = Some Freeable;
       erased_contents: forall b ofs,
-          erased_memval (ZMap.get ofs ((Mem.mem_contents m) # b))
+          memval_erasure (ZMap.get ofs ((Mem.mem_contents m) # b))
                         (ZMap.get ofs ((Mem.mem_contents m') # b));
       erased_nb: Mem.nextblock m = Mem.nextblock m'
     }.
 
-  Lemma erasedMem_restr:
+  Lemma mem_erasure_restr:
     forall m m' pmap (Hlt: permMapLt pmap (getMaxPerm m)),
-      erasedMem m m' ->
-      erasedMem (restrPermMap Hlt) m'.
+      mem_erasure m m' ->
+      mem_erasure (restrPermMap Hlt) m'.
   Proof.
     intros.
     inversion H.
     constructor; auto.
   Qed.
 
-  Lemma erasedMem_dilute_1:
+  Lemma mem_erasure_dilute_1:
     forall m m',
-      erasedMem m m' ->
-      erasedMem (setMaxPerm m) m'.
+      mem_erasure m m' ->
+      mem_erasure (setMaxPerm m) m'.
   Proof.
     intros.
     inversion H.
@@ -177,10 +828,10 @@ Module MemErasure.
 
   Lemma getN_erasure:
     forall m1 m2 b,
-      erasedMem m1 m2 ->
+      mem_erasure m1 m2 ->
       forall n ofs,
         Mem.range_perm m1 b ofs (ofs + Z_of_nat n) Cur Readable ->
-        erased_memval_list
+        memval_erasure_list
                      (Mem.getN n ofs (m1.(Mem.mem_contents)#b))
                      (Mem.getN n ofs (m2.(Mem.mem_contents)#b)).
   Proof.
@@ -193,20 +844,115 @@ Module MemErasure.
     apply IHn. red; intros; apply H0; omega.
   Qed.
 
+  Lemma proj_bytes_erasure:
+    forall vl vl',
+      memval_erasure_list vl vl' ->
+      forall bl,
+        proj_bytes vl = Some bl ->
+        proj_bytes vl' = Some bl.
+  Proof.
+    induction 1; simpl. congruence.
+    intros.
+    destruct mv; simpl in H; try discriminate.
+    subst.
+    destruct (proj_bytes mvl) eqn:Hproj; try discriminate.
+    inv H1.
+    erewrite IHmemval_erasure_list by eauto.
+    reflexivity.
+  Qed.
+
+  Lemma proj_bytes_not_erasure:
+    forall vl vl',
+      memval_erasure_list vl vl' ->
+      proj_bytes vl = None -> proj_bytes vl' <> None -> In Undef vl.
+  Proof.
+    induction 1; simpl; intros.
+    congruence.
+    destruct mv; simpl in *; subst; try discriminate; auto.
+    destruct (proj_bytes mvl) eqn:Hproj; try discriminate.
+    destruct (proj_bytes mvl'); try congruence.
+    right; eapply IHmemval_erasure_list; eauto; congruence.
+    destruct mv'; subst; congruence.
+  Qed.
+
+  Lemma check_value_erasure:
+    forall vl vl',
+      memval_erasure_list vl vl' ->
+      forall v v' q n,
+        check_value n v q vl = true ->
+        val_erasure v v' -> v <> Vundef ->
+        check_value n v' q vl' = true.
+  Proof.
+    induction 1; intros; destruct n; simpl in *; auto.
+    destruct mv; try discriminate.
+    simpl in H. destruct mv'; try discriminate.
+    destruct H as [? [? ?]]; subst.
+    
+    InvBooleans; assert (n = n1) by (apply beq_nat_true; auto). subst.
+    replace v1 with v'.
+    unfold proj_sumbool; rewrite ! dec_eq_true. rewrite <- beq_nat_refl. simpl; eauto.
+    destruct v0; simpl in *; subst; congruence.
+  Qed.
+
+  Lemma proj_value_erasure:
+    forall q vl1 vl2,
+      memval_erasure_list vl1 vl2 ->
+      val_erasure (proj_value q vl1) (proj_value q vl2).
+  Proof.
+    intros. unfold proj_value.
+    inv H; simpl; auto.
+    destruct mv; simpl in *; auto.
+    destruct mv'; try discriminate.
+    destruct H0 as [? [? ?]]; subst.
+    destruct (check_value (size_quantity_nat q) v q (Fragment v q1 n0 :: mvl)) eqn:B; auto.
+    destruct (Val.eq v Vundef). subst; auto.
+    assert (v = v0)
+      by (destruct v; simpl in *; congruence; auto).
+    subst.
+    erewrite check_value_erasure with (vl := (Fragment v0 q1 n0 :: mvl));
+      eauto with val_erasure.
+    simpl; auto.
+  Qed.
+  
+  Lemma load_result_erasure:
+    forall chunk v1 v2,
+      val_erasure v1 v2 ->
+      val_erasure (Val.load_result chunk v1) (Val.load_result chunk v2).
+  Proof.
+    intros. destruct v1; inv H; destruct chunk; simpl; econstructor; eauto.
+  Qed.
+  
   Lemma decode_val_erasure:
     forall vl1 vl2 chunk,
-      erased_memval_list vl1 vl2 ->
-      erased_val (decode_val chunk vl1) (decode_val chunk vl2).
+      memval_erasure_list vl1 vl2 ->
+      val_erasure (decode_val chunk vl1) (decode_val chunk vl2).
   Proof.
-    Admitted.
-  
+    intros. unfold decode_val.
+    destruct (proj_bytes vl1) as [bl1|] eqn:PB1.
+    exploit proj_bytes_erasure; eauto. intros PB2. rewrite PB2.
+    destruct chunk; simpl; auto.
+    assert (A: forall q fn,
+               val_erasure (Val.load_result chunk (proj_value q vl1))
+                          (match proj_bytes vl2 with
+                           | Some bl => fn bl
+                           | None => Val.load_result chunk (proj_value q vl2)
+                           end)).
+    { intros. destruct (proj_bytes vl2) as [bl2|] eqn:PB2.
+      rewrite proj_value_undef. destruct chunk; simpl; auto.
+      eapply proj_bytes_not_erasure; eauto. congruence.
+      apply load_result_erasure. apply proj_value_erasure; auto.
+    }
+    destruct chunk; simpl; eauto.
+  Qed.
+
+
   Lemma mem_load_erased:
     forall chunk m m' b ofs v
       (Hload: Mem.load chunk m b ofs = Some v)
-      (Herased: erasedMem m m'),
+      (Herased: mem_erasure m m'),
     exists v',
       Mem.load chunk m' b ofs = Some v' /\
-      erased_val v v'.
+      val_erasure v v'.
   Proof.
     intros.
     inversion Herased.
@@ -235,55 +981,19 @@ Module MemErasure.
     Opaque Mem.load.
   Qed.
 
-  Lemma inj_bytes_erasure :
-    forall (bl : seq.seq byte),
-      erased_memval_list (inj_bytes bl) (inj_bytes bl).
-  Admitted.
-
-  Lemma inj_value_erasure :
-    forall (v1 v2 : val) (q : quantity),
-      erased_val v1 v2 ->
-      erased_memval_list (inj_value q v1) (inj_value q v2).
-  Admitted.
-
-  Lemma repeat_Undef_erasure_self :
-    forall (n : nat),
-      erased_memval_list (list_repeat n Undef) (list_repeat n Undef).
-  Admitted.
-
-  Lemma repeat_Undef_inject_encode_val :
-    forall (chunk : memory_chunk) (v : val),
-      erased_memval_list (list_repeat (size_chunk_nat chunk) Undef)
-                         (encode_val chunk v).
-  Admitted.
-
-  Lemma encode_val_erasure:
-    forall (v1 v2 : val) (chunk : memory_chunk),
-      erased_val v1 v2 ->
-      erased_memval_list (encode_val chunk v1)
-                   (encode_val chunk v2).
-  Proof.
-    intros. 
-    destruct v1; inversion H; subst; simpl; destruct chunk;
-    auto using inj_bytes_erasure,  inj_value_erasure, repeat_Undef_erasure_self,
-    repeat_Undef_inject_encode_val.    
-    unfold encode_val. destruct v2; apply inj_value_erasure; auto.
-    unfold encode_val. destruct v2; apply inj_value_erasure; auto.
-  Qed.
-
   Lemma setN_erasure :
     forall (vl1 vl2 : seq.seq memval),
-      erased_memval_list vl1 vl2 ->
+      memval_erasure_list vl1 vl2 ->
       forall (p : Z) (c1 c2 : ZMap.t memval),
         (forall q : Z,
-            erased_memval (ZMap.get q c1) (ZMap.get q c2)) ->
+            memval_erasure (ZMap.get q c1) (ZMap.get q c2)) ->
         forall q : Z,
-          erased_memval (ZMap.get q (Mem.setN vl1 p c1))
+          memval_erasure (ZMap.get q (Mem.setN vl1 p c1))
                         (ZMap.get q (Mem.setN vl2 p c2)).
   Proof.
     induction 1; intros; simpl.
     auto.
-    apply IHerased_memval_list; auto.
+    apply IHmemval_erasure_list; auto.
     intros. erewrite ZMap.gsspec at 1. destruct (ZIndexed.eq q0 p). subst q0.
     rewrite ZMap.gss. auto.
     rewrite ZMap.gso. auto. unfold ZIndexed.t in *. omega.
@@ -292,10 +1002,10 @@ Module MemErasure.
   Lemma mem_store_erased:
     forall chunk m m' b ofs v v' m2
       (Hstore: Mem.store chunk m b ofs v = Some m2)
-      (Herased: erasedMem m m')
-      (Herased_val: erased_val v v') ,
+      (Herased: mem_erasure m m')
+      (Hval_erasure: val_erasure v v') ,
     exists m2', Mem.store chunk m' b ofs v' = Some m2'
-           /\ erasedMem m2 m2'.
+           /\ mem_erasure m2 m2'.
   Proof.
     intros.
     destruct Herased.
@@ -333,63 +1043,244 @@ Module MemErasure.
       rewrite ! PMap.gsspec.
       destruct (peq b0 b). subst b0.
       apply setN_erasure.
-      apply encode_val_erasure; auto. intros. eauto.
+      apply val_erasure_encode_val; auto. intros. eauto.
       eauto.
     - erewrite Mem.nextblock_store with (m1 := m) by eauto.
       erewrite Mem.nextblock_store with (m2 := m2') (m1 := m') by eauto.
       eauto.
   Qed.
+
+  Lemma mem_loadv_erased:
+    forall chunk m m' vptr v
+      (Hload: Mem.loadv chunk m vptr = Some v)
+      (Herased: mem_erasure m m'),
+    exists v',
+      Mem.loadv chunk m' vptr = Some v' /\
+      val_erasure v v'.
+  Proof.
+    intros.
+    destruct vptr; try discriminate.
+    simpl in *.
+    eapply mem_load_erased; eauto.
+  Qed.
+    
+  Lemma mem_storev_erased:
+    forall chunk m m' vptr v v' m2
+      (Hstore: Mem.storev chunk m vptr v = Some m2)
+      (Herased: mem_erasure m m')
+      (Hval_erasure: val_erasure v v') ,
+    exists m2', Mem.storev chunk m' vptr v' = Some m2'
+           /\ mem_erasure m2 m2'.
+  Proof.
+    intros.
+    destruct vptr; try discriminate.
+    simpl in *.
+    eapply mem_store_erased; eauto.
+  Qed.
+  
+  Lemma mem_erasure_valid_pointer:
+    forall m m' b ofs,
+      mem_erasure m m' ->
+      Mem.valid_pointer m b ofs ->
+      Mem.valid_pointer m' b ofs.
+  Proof.
+    intros.
+    unfold Mem.valid_pointer in *.
+    destruct H.
+    destruct Mem.perm_dec; try by exfalso.
+    assert (Mem.valid_block m' b).
+    { destruct (valid_block_dec m' b); auto.
+      unfold Mem.valid_block in *.
+      rewrite <- erased_nb0 in n.
+      eapply Mem.nextblock_noaccess with (ofs := ofs) (k := Cur) in n.
+      unfold Mem.perm in p.
+      clear H0.
+      rewrite n in p.
+      simpl in p.
+        by exfalso.
+    }
+    specialize (perm_le0 _ ofs Cur H).
+    unfold is_true.
+    apply proj_sumbool_is_true.
+    unfold Mem.perm.
+    rewrite perm_le0.
+    simpl; constructor.
+  Qed.
+
+  Lemma mem_erasure_valid_pointer_guard:
+    forall m m' b ofs ofs',
+      mem_erasure m m' ->
+      Mem.valid_pointer m' b ofs
+      || Mem.valid_pointer m' b ofs' = false ->
+      Mem.valid_pointer m b ofs
+      || Mem.valid_pointer m b ofs'= false.
+  Proof.
+    intros.
+    apply orb_false_iff in H0. destruct H0.
+    apply orb_false_iff.
+    split;
+      match goal with
+      | [|- Mem.valid_pointer m b ?Ofs = _] =>
+        destruct (Mem.valid_pointer m b Ofs) eqn:Hptr
+      end; auto;
+      eapply mem_erasure_valid_pointer in Hptr; eauto.
+  Qed.
+
+  Lemma val_erasure_cmpu:
+    forall v1 v2 v1' v2' m m' cmp
+      (Hval_erasure: val_erasure v1 v1')
+      (Hval_erasure2: val_erasure v2 v2')
+      (Hmem: mem_erasure m m'),
+      val_erasure (Val.cmpu (Mem.valid_pointer m) cmp v1 v2)
+                  (Val.cmpu (Mem.valid_pointer m') cmp v1' v2').
+  Proof with eauto with val_erasure.
+    intros.
+    destruct v1,v2; simpl in *; inv Hval_erasure; auto;
+    unfold Val.cmpu, Val.cmpu_bool; simpl; eauto with val_erasure;
+    do 2 rewrite andb_if;
+    repeat match goal with
+           | [|- context[match ?Expr with | _ => _ end]] =>
+             destruct Expr eqn:?
+           end; simpl; eauto with val_erasure.
+    eapply mem_erasure_valid_pointer_guard in Heqb2; eauto.
+    congruence.
+    eapply mem_erasure_valid_pointer_guard in Heqb2; eauto.
+    congruence.
+    subst.
+    apply andb_false_iff in Heqb2.
+    destruct Heqb2 as [Heqb2 | Heqb2];
+      eapply mem_erasure_valid_pointer_guard in Heqb2; eauto;
+      congruence.
+    apply andb_false_iff in Heqb2.
+    eapply mem_erasure_valid_pointer in Heqb1; eauto.
+    eapply mem_erasure_valid_pointer in Heqb0; eauto.
+    destruct Heqb2 as [Heqb2 | Heqb2];
+      congruence.
+  Qed.
+
+  Lemma storev_pointer:
+    forall chunk m vptr v m',
+      Mem.storev chunk m vptr v = Some m' ->
+      isPointer vptr.
+  Proof.
+    intros. destruct vptr; simpl in *; try discriminate.
+    auto.
+  Qed.
+
+  Lemma loadv_pointer:
+    forall chunk m vptr v,
+      Mem.loadv chunk m vptr = Some v ->
+      isPointer vptr.
+  Proof.
+    intros. destruct vptr; simpl in *; try discriminate.
+    auto.
+  Qed.
+
+  Lemma loadbytes_erasure:
+    forall m m' b ofs sz bytes
+      (Hmem_erasure: mem_erasure m m')
+      (Hloadbytes: Mem.loadbytes m b ofs sz = Some bytes),
+    exists bytes',
+      Mem.loadbytes m' b ofs sz = Some bytes' /\
+      memval_erasure_list bytes bytes'.
+  Proof.
+    intros.
+    Transparent Mem.loadbytes.
+    unfold Mem.loadbytes in *.
+    destruct (Mem.range_perm_dec m b ofs (ofs + sz) Cur Readable).
+    inv Hloadbytes.
+    exists (Mem.getN (nat_of_Z sz) ofs (m'.(Mem.mem_contents)#b)).
+    split. apply pred_dec_true.
+    unfold Mem.range_perm in r.
+    intros ofs' Hrange.
+    specialize (r _ Hrange).
+    assert (Mem.valid_block m' b).
+    { destruct (valid_block_dec m' b); auto.
+      destruct Hmem_erasure.
+      unfold Mem.valid_block in *.
+      rewrite <- erased_nb0 in n.
+      apply Mem.nextblock_noaccess with (ofs := ofs') (k := Cur) in n.
+      unfold Mem.perm in r.
+      rewrite n in r. simpl in r; by exfalso.
+    }
+    apply (perm_le Hmem_erasure) with (ofs := ofs') (k := Cur) in H.
+    unfold Mem.perm. rewrite H. simpl; constructor.
+    apply getN_erasure; auto.
+    destruct (zle 0 sz). rewrite nat_of_Z_eq; auto. omega.
+    rewrite nat_of_Z_neg. simpl. red; intros; omegaContradiction. omega.
+    discriminate.
+  Qed.
+    
+  Lemma mem_erasure_idempotent:
+    forall m m',
+      mem_erasure m m' ->
+      mem_erasure m (erasePerm m').
+  Proof.
+    intros.
+    destruct H.
+    constructor; auto.
+    intros.
+    unfold Mem.valid_block in *.
+    unfold Mem.nextblock, erasePerm in H.
+    eapply erasePerm_V with (ofs := ofs) (k := k) in H.
+    unfold permission_at in *.
+    auto.
+  Qed.
+  
+  Hint Resolve mem_erasure_idempotent mem_erasure_dilute_1
+       mem_erasure_restr: mem_erasure.
   
 End MemErasure.
 
 (** Erasure of cores *)
 Module Type CoreErasure (SEM: Semantics).
-  Import SEM ValErasure MemErasure event_semantics.
+  Import SEM ValErasure MemErasure TraceErasure event_semantics.
   
-  Parameter erasedCores : C -> C -> Prop.
-  Parameter erasedCores_refl: forall c, erasedCores c c.
+  Parameter core_erasure : C -> C -> Prop.
+  Parameter core_erasure_refl: forall c, core_erasure c c.
 
   Parameter at_external_erase:
-    forall c c' (Herase: erasedCores c c'),
+    forall c c' (Herase: core_erasure c c'),
       match at_external Sem c, at_external Sem c' with
       | Some (ef, sig, vs), Some (ef', sig', vs') =>
-        ef = ef' /\ sig = sig' /\ erased_val_list vs vs'
+        ef = ef' /\ sig = sig' /\ val_erasure_list vs vs'
       | None, None => True
       | _, _ => False
       end.
 
   Parameter after_external_erase:
     forall v v' c c' c2
-      (HeraseCores: erasedCores c c')
-      (HeraseVal: erased_val v v')
+      (HeraseCores: core_erasure c c')
+      (HeraseVal: val_erasure v v')
       (Hafter_external: after_external SEM.Sem (Some v) c = Some c2),
     exists c2',
       after_external SEM.Sem (Some v') c' = Some c2' /\
-      erasedCores c2 c2'.
+      core_erasure c2 c2'.
   
   Parameter erasure_initial_core:
     forall ge v arg v' arg' c
-      (Hv: erased_val v v')
-      (Harg: erased_val arg arg')
+      (Hv: val_erasure v v')
+      (Harg: val_erasure arg arg')
       (Hinit: initial_core Sem ge v [:: arg] = Some c),
       initial_core Sem ge v' [:: arg'] = Some c.
   
   Parameter halted_erase:
     forall c c'
-      (HeraseCores: erasedCores c c')
+      (HeraseCores: core_erasure c c')
       (Hhalted: halted SEM.Sem c),
       halted SEM.Sem c'.
 
   Parameter evstep_erase:
     forall ge c1 c1' c2 ev m1 m1' m2
-      (HeraseCores: erasedCores c1 c1')
-      (HerasedMem: erasedMem m1 m1')
+      (HeraseCores: core_erasure c1 c1')
+      (Hmem_erasure: mem_erasure m1 m1')
       (Hstep: ev_step Sem ge c1 m1 ev c2 m2),
-    exists c2' m2',
-      ev_step Sem ge c1' m1' ev c2' m2' /\
-      erasedCores c2 c2' /\ erasedMem m2 (erasePerm m2').
+    exists c2' m2' ev',
+      ev_step Sem ge c1' m1' ev' c2' m2' /\
+      core_erasure c2 c2' /\ mem_erasure m2 (erasePerm m2') /\
+      mem_event_list_erasure ev ev'.
 
-  Hint Resolve erasedCores_refl : erased.
+  Hint Resolve core_erasure_refl : erased.
   
 End CoreErasure.
 
@@ -399,32 +1290,32 @@ Module ThreadPoolErasure (SEM: Semantics)
   Import ValErasure CE
          Machines DryMachine ThreadPool.
   
-  Definition erasedCtl c c' : Prop :=
+  Definition ctl_erasure c c' : Prop :=
     match c, c' with
     | Kinit vf arg, Kinit vf' arg' =>
-      erased_val vf vf' /\ erased_val arg arg'
+      val_erasure vf vf' /\ val_erasure arg arg'
     | Krun c, Krun c' =>
-      erasedCores c c'
+      core_erasure c c'
     | Kblocked c, Kblocked c' =>
-      erasedCores c c'
+      core_erasure c c'
     | Kresume c arg, Kresume c' arg' =>
-      erasedCores c c' /\ arg = arg'
+      core_erasure c c' /\ arg = arg'
     (*we don't use this and our semantics are strange*)
     | _, _  => False
     end.
 
-  Inductive erased_threadPool tp (tp' : ErasedMachine.ThreadPool.t) :=
+  Inductive threadPool_erasure tp (tp' : ErasedMachine.ThreadPool.t) :=
   | ErasedPool :
       num_threads tp = ErasedMachine.ThreadPool.num_threads tp' ->
       (forall i (cnti: containsThread tp i)
          (cnti': ErasedMachine.ThreadPool.containsThread tp' i),
-          erasedCtl (getThreadC cnti)
+          ctl_erasure (getThreadC cnti)
                     (ErasedMachine.ThreadPool.getThreadC cnti')) ->
-      erased_threadPool tp tp'.
+      threadPool_erasure tp tp'.
 
   Lemma erasedPool_contains:
     forall tp1 tp1' 
-      (HerasedPool: erased_threadPool tp1 tp1') i,
+      (HerasedPool: threadPool_erasure tp1 tp1') i,
       containsThread tp1 i <-> ErasedMachine.ThreadPool.containsThread tp1' i.
   Proof.
     intros.
@@ -434,16 +1325,16 @@ Module ThreadPoolErasure (SEM: Semantics)
     split; auto.
   Qed.
 
-  Lemma erasedCtl_refl:
-    forall c, erasedCtl c c.
-  Proof with eauto with erased.
+  Lemma ctl_erasure_refl:
+    forall c, ctl_erasure c c.
+  Proof with eauto with val_erasure erased.
     destruct c; simpl...
   Qed.
   
   Lemma erased_updLockSet:
     forall tp tp' addr addr' rmap rmap',
-      erased_threadPool tp tp' ->
-      erased_threadPool (updLockSet tp addr rmap)
+      threadPool_erasure tp tp' ->
+      threadPool_erasure (updLockSet tp addr rmap)
                         (ErasedMachine.ThreadPool.updLockSet tp' addr' rmap').
   Proof.
     intros.
@@ -454,9 +1345,9 @@ Module ThreadPoolErasure (SEM: Semantics)
   Lemma erased_updThread:
     forall tp tp' i (cnti: containsThread tp i)
       (cnti': ErasedMachine.ThreadPool.containsThread tp' i) c c' pmap pmap',
-      erased_threadPool tp tp' ->
-      erasedCtl c c' ->
-      erased_threadPool (updThread cnti c pmap)
+      threadPool_erasure tp tp' ->
+      ctl_erasure c c' ->
+      threadPool_erasure (updThread cnti c pmap)
                         (ErasedMachine.ThreadPool.updThread cnti' c' pmap').
   Proof.
     intros.
@@ -473,12 +1364,12 @@ Module ThreadPoolErasure (SEM: Semantics)
   Lemma erased_addThread:
     forall tp tp' i (cnti: containsThread tp i)
       (cnti': ErasedMachine.ThreadPool.containsThread tp' i) v arg v' arg' pmap pmap',
-      erased_threadPool tp tp' ->
-      erased_val v v' ->
-      erased_val arg arg' ->
-      erased_threadPool (addThread tp v arg pmap)
+      threadPool_erasure tp tp' ->
+      val_erasure v v' ->
+      val_erasure arg arg' ->
+      threadPool_erasure (addThread tp v arg pmap)
                         (ErasedMachine.ThreadPool.addThread tp' v arg pmap').
-  Proof with eauto with erased.
+  Proof with eauto with val_erasure erased.
     intros.
     inversion H.
     constructor.
@@ -504,8 +1395,8 @@ Module ThreadPoolErasure (SEM: Semantics)
   
   Lemma erased_remLockSet:
     forall tp tp' addr addr',
-      erased_threadPool tp tp' ->
-      erased_threadPool (remLockSet tp addr)
+      threadPool_erasure tp tp' ->
+      threadPool_erasure (remLockSet tp addr)
                         (ErasedMachine.ThreadPool.remLockSet tp' addr').
   Proof.
     intros.
@@ -524,7 +1415,7 @@ Module SCErasure (SEM: Semantics)
        (AsmContext: AsmContext SEM Machines)
        (CE : CoreErasure SEM).
   Module ThreadPoolErasure := ThreadPoolErasure SEM Machines CE.
-  Import ValErasure MemErasure CE ThreadPoolErasure.
+  Import ValErasure MemErasure TraceErasure CE ThreadPoolErasure.
   Import Machines DryMachine ThreadPool AsmContext.
 
   Import event_semantics.
@@ -533,42 +1424,42 @@ Module SCErasure (SEM: Semantics)
   
   Lemma syncStep_erase:
     forall ge tp1 tp1' m1 m1' tp2 m2 i ev
-      (HerasePool: erased_threadPool tp1 tp1')
+      (HerasePool: threadPool_erasure tp1 tp1')
       (cnti: containsThread tp1 i)
       (cnti': ErasedMachine.ThreadPool.containsThread tp1' i)
-      (HerasedMem: erasedMem m1 m1')
+      (Hmem_erasure: mem_erasure m1 m1')
       (Hcomp1: mem_compatible tp1 m1)
       (Hcomp1': ErasedMachine.mem_compatible tp1' m1')
       (Hstep: syncStep ge cnti Hcomp1 tp2 m2 ev),
     exists tp2' m2',
       ErasedMachine.syncStep ge cnti' Hcomp1' tp2' m2' ev /\
-      erased_threadPool tp2 tp2' /\ erasedMem m2 m2'.
-  Proof with eauto with erased.
+      threadPool_erasure tp2 tp2' /\ mem_erasure m2 m2'.
+  Proof with eauto with val_erasure erased.
     intros.
-    Hint Resolve erasedMem_restr : erased.
+    Hint Resolve mem_erasure_restr : erased.
     inversion HerasePool as [Hnum Hthreads].
     specialize (Hthreads _ cnti cnti').      
     inversion Hstep; subst;
     match goal with
-    | [H: erasedCtl ?Expr1 ?Expr2, H1: ?Expr1 = _ |- _] =>
+    | [H: ctl_erasure ?Expr1 ?Expr2, H1: ?Expr1 = _ |- _] =>
       rewrite H1 in H; simpl in H;
       destruct Expr2 eqn:?
     end; try (by exfalso);
     try match goal with
         | [H: Mem.load _ _ _ _ = Some _ |- _] =>
-          eapply mem_load_erased in H; eauto with erased;
+          eapply mem_load_erased in H; eauto with val_erasure erased;
           destruct Hload as [? [Hload ?]]
         end;
     try match goal with
         | [H: Mem.store _ _ _ _ _ = Some _ |- _] =>
-          eapply mem_store_erased in H; eauto with erased;
-          destruct Hstore as [m2' [Hstore HerasedMem']]
+          eapply mem_store_erased in H; eauto with val_erasure erased;
+          destruct Hstore as [m2' [Hstore Hmem_erasure']]
         end;
     try match goal with
         | [|- _ <> Vundef] => intro Hcontra; discriminate
         end;
     match goal with
-    | [H: at_external _ _ = _, H1: erasedCores _ _ |- _] =>
+    | [H: at_external _ _ = _, H1: core_erasure _ _ |- _] =>
       pose proof (at_external_erase H1);
         match goal with
         | [H2: match at_external _ _ with _ => _ end |- _] =>
@@ -581,10 +1472,10 @@ Module SCErasure (SEM: Semantics)
     end;
     repeat match goal with
            | [H: _ /\ _ |- _] => destruct H
-           | [H: erased_val_list _ _ |- _] =>
+           | [H: val_erasure_list _ _ |- _] =>
              inv H
-           | [H: erased_val (Vptr _ _) _ |- _] => inv H
-           | [H:erased_val (Vint _) _ |- _] => inv H
+           | [H: val_erasure (Vptr _ _) _ |- _] => inv H
+           | [H:val_erasure (Vint _) _ |- _] => inv H
            end; subst.
     - exists (ErasedMachine.ThreadPool.updThreadC cnti' (Kresume c0 Vundef)), m2'.
       split; [econstructor; eauto | split; eauto].
@@ -643,7 +1534,7 @@ Module SCErasure (SEM: Semantics)
           erewrite <- @ErasedMachine.ThreadPool.gsoThreadCC with (cntj := cntj00')
             by eauto.
           inversion HerasePool; eauto.
-      + (*case j is the just addded thread *)
+      + (*case j is the just added thread *)
         subst.
         erewrite gssAddCode by (unfold latestThread; reflexivity).
         erewrite ErasedMachine.ThreadPool.gssAddCode
@@ -705,15 +1596,16 @@ Module SCErasure (SEM: Semantics)
              apply cntUpdate' in H2;
                assert (H1 = H2) by (by eapply cnt_irr); subst H2
            end.
+  
   Lemma startStep_erasure:
     forall ge tp1 tp1' tp2 i
-      (HerasePool: erased_threadPool tp1 tp1')
+      (HerasePool: threadPool_erasure tp1 tp1')
       (cnti: containsThread tp1 i)
       (cnti': ErasedMachine.ThreadPool.containsThread tp1' i)
       (Hstep: FineConc.start_thread ge cnti tp2),
     exists tp2',
       SC.start_thread ge cnti' tp2' /\
-      erased_threadPool tp2 tp2'.
+      threadPool_erasure tp2 tp2'.
   Proof.
     intros.
     inversion HerasePool as [Hnum Hthreads].
@@ -721,15 +1613,15 @@ Module SCErasure (SEM: Semantics)
     inversion Hstep; subst.
     pf_cleanup;
       match goal with
-        [H: erasedCtl ?Expr1 ?Expr2, H1: ?Expr1 = _ |- _] =>
+        [H: ctl_erasure ?Expr1 ?Expr2, H1: ?Expr1 = _ |- _] =>
         rewrite H1 in H; simpl in H;
         destruct Expr2 eqn:?
       end; try (by exfalso).
     repeat match goal with
            | [H: _ /\ _ |- _] => destruct H
-           | [H: erased_val_list _ _ |- _] =>
+           | [H: val_erasure_list _ _ |- _] =>
              inv H
-           | [H: erased_val (Vptr _ _) _ |- _] => inv H
+           | [H: val_erasure (Vptr _ _) _ |- _] => inv H
            end; subst.
     eapply erasure_initial_core in Hinitial; eauto.
     exists (ErasedMachine.ThreadPool.updThreadC cnti' (Krun c_new)).
@@ -740,7 +1632,7 @@ Module SCErasure (SEM: Semantics)
     + subst.
       rewrite gssThreadCC.
       rewrite ErasedMachine.ThreadPool.gssThreadCC.
-      simpl. apply erasedCores_refl.
+      simpl. apply core_erasure_refl.
     +
       assert (cntj0' := ErasedMachine.ThreadPool.cntUpdateC' _ _ cntj').
       assert (cntj0 := cntUpdateC' _ _ cntj).
@@ -752,13 +1644,13 @@ Module SCErasure (SEM: Semantics)
 
   Lemma resumeStep_erasure:
     forall tp1 tp1' tp2 i
-      (HerasePool: erased_threadPool tp1 tp1')
+      (HerasePool: threadPool_erasure tp1 tp1')
       (cnti: containsThread tp1 i)
       (cnti': ErasedMachine.ThreadPool.containsThread tp1' i)
       (Hstep: FineConc.resume_thread cnti tp2),
     exists tp2',
       SC.resume_thread cnti' tp2' /\
-      erased_threadPool tp2 tp2'.
+      threadPool_erasure tp2 tp2'.
   Proof.
     intros.
     inversion HerasePool as [Hnum Hthreads].
@@ -766,7 +1658,7 @@ Module SCErasure (SEM: Semantics)
     inversion Hstep; subst.
     pf_cleanup;
       match goal with
-        [H: erasedCtl ?Expr1 ?Expr2, H1: ?Expr1 = _ |- _] =>
+        [H: ctl_erasure ?Expr1 ?Expr2, H1: ?Expr1 = _ |- _] =>
         rewrite H1 in H; simpl in H;
         destruct Expr2 eqn:?
       end; try (by exfalso).
@@ -778,8 +1670,8 @@ Module SCErasure (SEM: Semantics)
     destruct p as [[? ?] ?].
     destruct H as [? [? ?]]; subst.
     eapply after_external_erase with (v' := Vint Int.zero) in Hafter_external;
-      eauto with erased.
-    destruct Hafter_external as [c2' [Hafter_external' HerasedCores']].
+      eauto with val_erasure erased.
+    destruct Hafter_external as [c2' [Hafter_external' Hcore_erasure']].
     exists (ErasedMachine.ThreadPool.updThreadC cnti' (Krun c2')).
     split.
     eapply SC.ResumeThread with (c := c0); simpl in *; eauto.
@@ -803,13 +1695,13 @@ Module SCErasure (SEM: Semantics)
   
   Lemma suspendStep_erasure:
     forall tp1 tp1' tp2 i
-      (HerasePool: erased_threadPool tp1 tp1')
+      (HerasePool: threadPool_erasure tp1 tp1')
       (cnti: containsThread tp1 i)
       (cnti': ErasedMachine.ThreadPool.containsThread tp1' i)
       (Hstep: FineConc.suspend_thread cnti tp2),
     exists tp2',
       SC.suspend_thread cnti' tp2' /\
-      erased_threadPool tp2 tp2'.
+      threadPool_erasure tp2 tp2'.
   Proof.
     intros.
     inversion HerasePool as [Hnum Hthreads].
@@ -817,7 +1709,7 @@ Module SCErasure (SEM: Semantics)
     inversion Hstep; subst.
     pf_cleanup;
       match goal with
-        [H: erasedCtl ?Expr1 ?Expr2, H1: ?Expr1 = _ |- _] =>
+        [H: ctl_erasure ?Expr1 ?Expr2, H1: ?Expr1 = _ |- _] =>
         rewrite H1 in H; simpl in H;
         destruct Expr2 eqn:?
       end; try (by exfalso).
@@ -850,7 +1742,7 @@ Module SCErasure (SEM: Semantics)
 
   Lemma haltStep_erasure:
     forall tp1 tp1' i
-      (HerasePool: erased_threadPool tp1 tp1')
+      (HerasePool: threadPool_erasure tp1 tp1')
       (cnti: containsThread tp1 i)
       (cnti': ErasedMachine.ThreadPool.containsThread tp1' i)
       (Hstep: threadHalted cnti),
@@ -870,18 +1762,19 @@ Module SCErasure (SEM: Semantics)
     econstructor; eauto.
   Qed.
 
-   Lemma threadStep_erase:
+  Lemma threadStep_erase:
     forall ge tp1 tp1' m1 m1' tp2 m2 i ev
-      (HerasePool: erased_threadPool tp1 tp1')
+      (HerasePool: threadPool_erasure tp1 tp1')
       (cnti: containsThread tp1 i)
       (cnti': ErasedMachine.ThreadPool.containsThread tp1' i)
-      (HerasedMem: erasedMem m1 m1')
+      (Hmem_erasure: mem_erasure m1 m1')
       (Hcomp1: mem_compatible tp1 m1)
       (Hcomp1': ErasedMachine.mem_compatible tp1' m1')
       (Hstep: threadStep ge cnti Hcomp1 tp2 m2 ev),
-    exists tp2' m2',
-      ErasedMachine.threadStep ge cnti' Hcomp1' tp2' m2' ev /\
-      erased_threadPool tp2 tp2' /\ erasedMem m2 (erasePerm m2').
+    exists tp2' m2' ev',
+      ErasedMachine.threadStep ge cnti' Hcomp1' tp2' m2' ev' /\
+      threadPool_erasure tp2 tp2' /\ mem_erasure m2 (erasePerm m2') /\
+      mem_event_list_erasure ev ev'.
   Proof.
     intros.
     inversion HerasePool as [Hnum Hthreads].
@@ -889,14 +1782,15 @@ Module SCErasure (SEM: Semantics)
     inversion Hstep; subst.
     pf_cleanup;
       match goal with
-        [H: erasedCtl ?Expr1 ?Expr2, H1: ?Expr1 = _ |- _] =>
+        [H: ctl_erasure ?Expr1 ?Expr2, H1: ?Expr1 = _ |- _] =>
         rewrite H1 in H; simpl in H;
         destruct Expr2 eqn:?
       end; try (by exfalso).
-    eapply erasedMem_restr with (Hlt := Hcomp1 i cnti) in HerasedMem.
+    eapply mem_erasure_restr with (Hlt := Hcomp1 i cnti) in Hmem_erasure.
     eapply evstep_erase in Hcorestep; eauto.
-    destruct Hcorestep as (c2' & m2' & Hevstep' & HerasedCores' & HerasedMem').
-    exists (ErasedMachine.ThreadPool.updThreadC cnti' (Krun c2')), m2'.
+    destruct Hcorestep as (c2' & m2' & ev' & Hevstep' & Hcore_erasure'
+                           & Hmem_erasure' & Hev_erasure).
+    exists (ErasedMachine.ThreadPool.updThreadC cnti' (Krun c2')), m2', ev'.
     split; eauto.
     econstructor; eauto.
     split; eauto.
@@ -920,16 +1814,17 @@ Module SCErasure (SEM: Semantics)
   Notation scstep := (corestep sc_semantics).
 
   (** A step on the FineConc machine can be matched by a step on the
-  SC machine producing the same event *)
+  SC machine producing an erased event *)
   Lemma sc_sim:
-    forall ge tp1 tp1' i U tr tr' m1 m1' tp2 m2
-      (HerasePool: erased_threadPool tp1 tp1')
-      (HerasedMem: erasedMem m1 m1')
-      (Hfstep: fstep ge (i :: U, tr, tp1) m1 (U, tr', tp2) m2),
-    exists tp2' m2',
-      scstep ge (i :: U, tr, tp1') m1' (U, tr', tp2') m2' /\
-      erased_threadPool tp2 tp2' /\ erasedMem m2 m2'.
-  Proof.
+    forall ge tp1 tp1' i U tr1 tr1' tr2 m1 m1' tp2 m2
+      (HerasePool: threadPool_erasure tp1 tp1')
+      (Hmem_erasure: mem_erasure m1 m1')
+      (Hfstep: fstep ge (i :: U, tr1, tp1) m1 (U, tr2, tp2) m2),
+    exists tp2' m2' tr2',
+      scstep ge (i :: U, tr1', tp1') m1' (U, tr2', tp2') m2' /\
+      threadPool_erasure tp2 tp2' /\ mem_erasure m2 m2' /\
+      (trace_erasure tr1 tr1' -> trace_erasure tr2 tr2').
+  Proof with eauto with trace_erasure mem_erasure.
     intros.
     inversion Hfstep; simpl in *; subst;
     inv HschedN;
@@ -942,34 +1837,34 @@ Module SCErasure (SEM: Semantics)
       by (unfold ErasedMachine.mem_compatible; auto).
     - assert (Hstep' := startStep_erasure HerasePool H Htstep).
       destruct Hstep' as [tp2' [Hstart' HerasePool']].
-      exists tp2', m1'.
+      exists tp2', m1', tr1'.
       split. econstructor 1; simpl; eauto.
       split; eauto.
     - assert (Hstep' := resumeStep_erasure HerasePool H Htstep).
       destruct Hstep' as [tp2' [Hstart' HerasePool']].
-      exists tp2', m1'.
+      exists tp2', m1', tr1'.
       split. econstructor 2; simpl; eauto.
       split; eauto.
-    - assert (Htstep' := threadStep_erase HerasePool H HerasedMem Hcomp1' Htstep).
-      destruct Htstep' as [tp2' [m2' [Htstep' [HerasePool' HerasedMem']]]].
-      exists tp2', (erasePerm m2').
+    - assert (Htstep' := threadStep_erase HerasePool H Hmem_erasure Hcomp1' Htstep).
+      destruct Htstep' as (tp2' & m2' & ev' & Htstep' & HerasePool'
+                           & Hmem_erasure' & Htr_erasure').
+      exists tp2', (erasePerm m2'), (tr1' ++ map [eta Events.internal tid] ev').
       split.
       eapply SC.thread_step; eauto.
-      split; eauto.
-      eapply erasedMem_dilute_1; eauto.
+      split...
     - assert (Hstep' := suspendStep_erasure HerasePool H Htstep).
       destruct Hstep' as [tp2' [Hstart' HerasePool']].
-      exists tp2', m1'.
+      exists tp2', m1', tr1'.
       split. econstructor 4; simpl; eauto.
       split; eauto.
-    - assert (Hstep' := syncStep_erase HerasePool H HerasedMem Hcomp1' Htstep).
-      destruct Hstep' as [tp2' [m2' [Hstep' [HerasePool' HerasedMem']]]].
-      exists tp2', m2'.
+    - assert (Hstep' := syncStep_erase HerasePool H Hmem_erasure Hcomp1' Htstep).
+      destruct Hstep' as (tp2' & m2' & Hstep' & HerasePool' & Hmem_erasure').
+      exists tp2', m2', (tr1' ++ [:: Events.external tid ev]).
       split.
       eapply SC.sync_step; eauto.
-      split; eauto.
+      split...
     - eapply haltStep_erasure with (cnti' := H) in Hhalted; eauto.
-      exists tp1', m1';
+      exists tp1', m1', tr1';
         split; eauto.
       econstructor 6; simpl; eauto.
     - assert (~ ErasedMachine.ThreadPool.containsThread tp1' tid).
@@ -979,7 +1874,7 @@ Module SCErasure (SEM: Semantics)
         rewrite <- Hnum in Hcontra.
         auto.
       }
-      exists tp1', m1'.
+      exists tp1', m1',tr1'.
       split.
       econstructor 7; simpl; eauto.
       split; eauto.
@@ -1068,7 +1963,7 @@ Module SCErasure (SEM: Semantics)
     forall f arg U tpsc tpf
       (HinitSC: sc_init f arg = Some (U, [::], tpsc))
       (HinitF: tpf_init f arg = Some (U, [::], tpf)),
-      erased_threadPool tpf tpsc.
+      threadPool_erasure tpf tpsc.
   Proof.
     intros.
     unfold sc_init, tpf_init in *.
@@ -1083,47 +1978,51 @@ Module SCErasure (SEM: Semantics)
     econstructor. simpl; eauto.
     intros. 
     simpl.
-    apply erasedCores_refl; auto.
+    apply core_erasure_refl; auto.
   Qed.
 
   (** Any execution of the FineConc machine resulting in some trace
-    tr' can be matched by an execution of the SC machine with the
-    same trace*)
+    tr' can be matched by an execution of the SC machine with an
+    erased trace *)
   Lemma execution_sim:
-    forall U U' tpf tpf' mf mf' tpsc msc tr tr' 
+    forall U U' tpf tpf' mf mf' tpsc msc tr tr' trsc 
       (Hexec: fine_execution (U, tr, tpf) mf (U', tr', tpf') mf')
-      (HerasedPool: erased_threadPool tpf tpsc)
-      (HerasedMem: erasedMem mf msc),
-    exists tpsc' msc',
-      sc_execution (U, tr, tpsc) msc (U', tr', tpsc') msc' /\
-      erased_threadPool tpf' tpsc' /\ erasedMem mf' msc'.
-  Proof.
+      (HerasedPool: threadPool_erasure tpf tpsc)
+      (Hmem_erasure: mem_erasure mf msc),
+    exists tpsc' msc' trsc',
+      sc_execution (U, trsc, tpsc) msc (U', trsc', tpsc') msc' /\
+      threadPool_erasure tpf' tpsc' /\ mem_erasure mf' msc' /\
+      (trace_erasure tr trsc -> trace_erasure tr' trsc').
+  Proof with eauto.
     intros U.
     induction U.
     - intros.
       inversion Hexec; subst.
-      exists tpsc, msc.
+      exists tpsc, msc, trsc.
       split.
       econstructor 1. simpl; auto.
-      split; auto.
+      split... 
     - intros.
       inversion Hexec; subst.
       + simpl in H5; by exfalso.
-      + eapply sc_sim in H8; eauto.
-        destruct H8 as (tpsc0 & msc0 & Hstep0 & HerasedPool0 & HerasedMem0).
-        specialize (IHU _ _ _ _ _ _ _ _ _ H9 HerasedPool0 HerasedMem0).
-        destruct IHU as (tpsc2' & msc2' & Hsexec & HerasedPool' & HerasedMem').
-        exists tpsc2', msc2'.
-        split; eauto.
-        econstructor; eauto.
+      + eapply sc_sim with (tr1' := trsc) in H8; eauto.
+        destruct H8 as (tpsc0 & msc0 & tr0 & Hstep0 & HerasedPool0
+                        & Hmem_erasure0 & Htrace_erasure0).
+        specialize (IHU _ _ _ _ _ _ _ _ _ tr0 H9 HerasedPool0
+                        Hmem_erasure0).
+        destruct IHU as (tpsc2' & msc2' & trsc2' & Hsexec & HerasedPool'
+                         & Hmem_erasure' & Htrace_erasure2').
+        exists tpsc2', msc2', trsc2'.
+        split...
+        econstructor...
   Qed.
 
   (** Safety of the SC machine*)
   Lemma fsafe_implies_scsafe:
     forall sched tpsc tpf mf msc
       (Hsafe: fsafe tpf mf sched (size sched).+1)
-      (HerasedPool: erased_threadPool tpf tpsc)
-      (HerasedMem: erasedMem mf msc),
+      (HerasedPool: threadPool_erasure tpf tpsc)
+      (Hmem_erasure: mem_erasure mf msc),
       sc_safe tpsc msc sched (size sched).+1.
   Proof.
     intro sched.
@@ -1135,8 +2034,11 @@ Module SCErasure (SEM: Semantics)
       inversion Hsafe; subst.
       simpl in H; by exfalso.
       simpl in *.
-      eapply sc_sim in H0; eauto.
-      destruct H0 as (tpsc2' & msc2' & Hstep & HerasedPool' & HerasedMem').
+      eapply fstep_trace_irr with (tr'' := [::]) in H0.
+      destruct H0 as [ev Hstep]. simpl in Hstep.
+      eapply sc_sim with (tr1' := [::]) in Hstep; eauto.
+      destruct Hstep as (tpsc2' & msc2' & ? & Hstep & HerasedPool'
+                         & Hmem_erasure' & ?).
       econstructor 3; eauto.
   Qed.
   
@@ -1150,25 +2052,33 @@ Module SCErasure (SEM: Semantics)
       (forall tpf' mf' tr,
           fine_execution (sched, [::], tpf) (DryMachine.diluteMem m)
                          ([::], tr, tpf') mf' ->
-          exists tpsc' msc',
+          exists tpsc' msc' tr',
             sc_execution (sched, [::], tpsc) (ErasedMachine.diluteMem m)
-                         ([::], tr, tpsc') msc' /\
-            erased_threadPool tpf' tpsc' /\ erasedMem mf' msc').
-  Proof.
+                         ([::], tr', tpsc') msc' /\
+            threadPool_erasure tpf' tpsc' /\ mem_erasure mf' msc' /\
+      trace_erasure tr tr').
+  Proof with eauto.
     intros.
     assert (HpoolErase := init_erasure _ _ HinitSC HinitF).
-    assert (HmemErase : erasedMem (diluteMem m) (ErasedMachine.diluteMem m)).
-    { econstructor; eauto.
+    assert (HmemErase : mem_erasure (diluteMem m) (ErasedMachine.diluteMem m)).
+    { eapply mem_erasure_dilute_1.
+      econstructor; eauto.
       intros.
       assert (Hvalid: Mem.valid_block m b)
         by (unfold Mem.valid_block, ErasedMachine.diluteMem, erasePerm in *;
              simpl in *; auto).
       assert (Hperm:= erasePerm_V ofs k Hvalid).
       unfold permission_at in Hperm; auto.
+      simpl.
+      intros.
+      eapply memval_erasure_refl.
     }
     split; first by (eapply fsafe_implies_scsafe; eauto).
     intros.
-    eapply execution_sim; eauto.
+    eapply execution_sim with (trsc := [::]) in H; eauto.
+    destruct H as (? & ? & ? & ?& ?& ? & Htrace_erasure).
+    specialize (Htrace_erasure ltac:(by constructor)).
+    do 3 eexists; split... 
   Qed.
 
 End SCErasure.
