concurrency/x86_safe.v
@@ -36,66 +36,78 @@ Set Bullet Behavior "Strict Subproofs".
 Module X86CoreErasure <: CoreErasure X86SEM.
   Import X86SEM ValErasure MemErasure event_semantics.
   
-  Definition erased_reg (r:PregEq.t) (rs rs' : regset) : Prop :=
-    erased_val (Pregmap.get r rs) (Pregmap.get r rs').
+  Definition reg_erasure (r:PregEq.t) (rs rs' : regset) : Prop :=
+    val_erasure (Pregmap.get r rs) (Pregmap.get r rs').
   
-  Definition erased_regs rs rs' : Prop :=
-    forall r, erased_reg r rs rs'.
+  Definition regs_erasure rs rs' : Prop :=
+    forall r, reg_erasure r rs rs'.
 
-  Definition erased_loader (l l' : load_frame) : Prop :=
+  Definition loader_erasure (l l' : load_frame) : Prop :=
     l = l'.
 
-  Definition erasedCores c c' :=
+  Definition core_erasure c c' :=
     match c, c' with
     | State rs loader, State rs' loader' =>
-      erased_regs rs rs' /\ erased_loader loader loader'
+      regs_erasure rs rs' /\ loader_erasure loader loader'
     | Asm_CallstateIn vf args tys retty, Asm_CallstateIn vf' args' tys' retty' =>
-      vf = vf' /\ erased_val_list args args' /\
+      vf = vf' /\ val_erasure_list args args' /\
       tys = tys' /\ retty = retty'
     | Asm_CallstateOut ef vals rs loader, Asm_CallstateOut ef' vals' rs' loader' =>
-      ef = ef' /\ erased_val_list vals vals'
-      /\ erased_regs rs rs' /\ erased_loader loader loader'
+      ef = ef' /\ val_erasure_list vals vals'
+      /\ regs_erasure rs rs' /\ loader_erasure loader loader'
     | _, _ => False
     end.
  
-  Lemma erased_regs_refl:
-    forall rs, erased_regs rs rs.
-  Proof with eauto with erased.
+  Lemma regs_erasure_refl:
+    forall rs, regs_erasure rs rs.
+  Proof with eauto with val_erasure.
     intros rs r;
-    unfold erased_reg...
+    unfold reg_erasure...
   Qed.
 
-  Lemma erased_loader_refl:
-    forall loader, erased_loader loader loader.
+  Lemma loader_erasure_refl:
+    forall loader, loader_erasure loader loader.
   Proof.
-    unfold erased_loader; auto.
+    unfold loader_erasure; auto.
   Qed.
   
-  Hint Immediate erased_regs_refl erased_loader_refl
-       erased_val_list_refl : erased.
+  Hint Immediate regs_erasure_refl loader_erasure_refl : regs_erasure.
+  Hint Immediate val_erasure_list_refl : val_erasure.
 
-  Lemma erasedCores_refl:
-    forall c, erasedCores c c.
-  Proof with eauto with erased.
+  Lemma core_erasure_refl:
+    forall c, core_erasure c c.
+  Proof with eauto with val_erasure regs_erasure.
     destruct c; simpl;
     repeat split...
   Qed.
 
-  Hint Immediate erasedCores_refl: erased.
+  Hint Immediate core_erasure_refl: regs_erasure.
   
-  Lemma erased_regs_set:
+  Lemma regs_erasure_set:
     forall rs rs' v v' r
-      (Hrs_ren: erased_regs rs rs')
-      (Hval: erased_val v v'),
-      erased_regs (rs # r <- v) (rs' # r <- v').
+      (Hrs_ren: regs_erasure rs rs')
+      (Hval: val_erasure v v'),
+      regs_erasure (rs # r <- v) (rs' # r <- v').
   Proof.
     intros.
     intros r'.
-    unfold erased_reg.
+    unfold reg_erasure.
     do 2 rewrite Pregmap.gsspec.
     destruct (Pregmap.elt_eq r' r); auto.
     eapply Hrs_ren.
   Qed.
+
+  Lemma regs_erasure_get:
+    forall rs rs' r,
+      regs_erasure rs rs' ->
+      val_erasure (rs r) (rs' r).
+  Proof.
+    intros.
+    unfold regs_erasure, reg_erasure in *. eauto.
+  Qed.
+  
+  Hint Resolve regs_erasure_get regs_erasure_refl regs_erasure_set : regs_erasure.
+  
 
   (*NOTE THIS IS DUPLICATED WITH X86_INJ*)
   Lemma set_regs_empty_1:
@@ -106,20 +118,19 @@ Module X86CoreErasure <: CoreErasure X86SEM.
     induction regs; by reflexivity.
   Qed.
   
-  Hint Resolve erased_regs_set : erased.
 
   (** ** Result about at_external, after_external and initial_core *)
   Lemma at_external_erase:
-    forall c c' (Herase: erasedCores c c'),
+    forall c c' (Herase: core_erasure c c'),
       match at_external Sem c, at_external Sem c' with
       | Some (ef, sig, vs), Some (ef', sig', vs') =>
-        ef = ef' /\ sig = sig' /\ erased_val_list vs vs'
+        ef = ef' /\ sig = sig' /\ val_erasure_list vs vs'
       | None, None => True
       | _, _ => False
       end.
   Proof.
     intros.
-    unfold erasedCores in *.
+    unfold core_erasure in *.
     destruct c, c'; try (by exfalso);
     repeat match goal with
     | [H: _ /\ _ |- _] => destruct H
@@ -128,17 +139,17 @@ Module X86CoreErasure <: CoreErasure X86SEM.
     destruct (BuiltinEffects.observableEF_dec f0); auto.
     split; auto.
     split; auto.
-    eapply erased_val_list_decode; eauto.
+    eapply val_erasure_list_decode; eauto.
   Qed.
 
   Lemma after_external_erase :
     forall v v' c c' c2
-      (HeraseCores: erasedCores c c')
-      (HeraseVal: erased_val v v')
+      (HeraseCores: core_erasure c c')
+      (HeraseVal: val_erasure v v')
       (Hafter_external: after_external X86SEM.Sem (Some v) c = Some c2),
     exists (c2' : state),
       after_external X86SEM.Sem (Some v') c' = Some c2' /\
-      erasedCores c2 c2'.
+      core_erasure c2 c2'.
   Proof.
     intros.
     unfold after_external in *.
@@ -146,33 +157,33 @@ Module X86CoreErasure <: CoreErasure X86SEM.
     unfold Asm_after_external in *.
     destruct c; try discriminate.
     inv Hafter_external.
-    unfold erasedCores in HeraseCores.
+    unfold core_erasure in HeraseCores.
     destruct c'; try by exfalso.
     destruct HeraseCores as (? & ? & ? &?); subst.
-    unfold erased_loader in H2; subst.
+    unfold loader_erasure in H2; subst.
     eexists; split; eauto.
     simpl.
-    split; [|unfold erased_loader; auto].      
+    split; [|unfold loader_erasure; auto].      
     destruct (loc_external_result (ef_sig f0)) as [|r' regs];
       simpl.
-    eapply erased_regs_set; eauto.
+    eapply regs_erasure_set; eauto.
     eapply H1.
     destruct (sig_res (ef_sig f0)) as [ty|];
       try destruct ty;
       simpl;
       try do 2 rewrite set_regs_empty_1;
-      repeat apply erased_regs_set; eauto;
+      repeat apply regs_erasure_set; eauto;
       try apply H1.
     destruct regs as [|r'' regs'']; simpl;
-    eauto with erased.
+    eauto with val_erasure regs_erasure.
     do 2 rewrite set_regs_empty_1;
-      eauto with erased.
+      eauto with regs_erasure val_erasure.
   Qed.
 
   Lemma erasure_initial_core:
     forall ge v arg v' arg' c
-      (Hv: erased_val v v')
-      (Harg: erased_val arg arg')
+      (Hv: val_erasure v v')
+      (Harg: val_erasure arg arg')
       (Hinit: initial_core Sem ge v [:: arg] = Some c),
       initial_core Sem ge v' [:: arg'] = Some c.
   Proof.
@@ -200,7 +211,7 @@ Module X86CoreErasure <: CoreErasure X86SEM.
 
   Lemma halted_erase:
     forall c c'
-      (HeraseCores: erasedCores c c')
+      (HeraseCores: core_erasure c c')
       (Hhalted: halted Sem c),
       halted Sem c'.
   Proof.
@@ -210,119 +221,686 @@ Module X86CoreErasure <: CoreErasure X86SEM.
     destruct c; try by exfalso.
     destruct c'; try by exfalso.
     destruct HeraseCores.
-    unfold erased_loader in H0. subst.
+    unfold loader_erasure in H0. subst.
     destruct loader0; try by exfalso.
     destruct (Val.eq (rs PC) Vundef).
     rewrite e in Hhalted.
     simpl in Hhalted; by exfalso.
-    pose proof (H PC). unfold erased_reg, Pregmap.get in H0.
-    erewrite <- erased_val_cmp_bool; eauto.
+    pose proof (H PC). unfold reg_erasure, Pregmap.get in H0.
+    erewrite <- val_erasure_cmp_bool; eauto.
     destruct (Val.cmp_bool Ceq (rs PC) Vzero); try by exfalso.
     destruct retty; try by exfalso.
     destruct t; auto.
     auto.
   Qed.
 
-  Lemma exec_instr_erased:
-    forall (g : genv) (fn : function) (i : instruction) (rs rs' rs2: regset)
-      (m m' m2 : mem)
-      (HeraseCores: erased_regs rs rs')
-      (HerasedMem: erasedMem m m')
-      (Hexec: exec_instr g fn i rs m = Next rs2 m2),
-    exists rs2' m2',
-      exec_instr g fn i rs' m' = Next rs2' m2' /\
-      erased_regs rs2 rs2' /\ erasedMem m2 (erasePerm m2').
- Admitted.
+  Lemma eval_testcond_erasure:
+    forall (c : testcond) rs rs'
+      (Hrs: regs_erasure rs rs'),
+      eval_testcond c rs <> None ->
+      eval_testcond c rs = eval_testcond c rs'.
+  Proof.
+    intros.
+    unfold eval_testcond in *.
+    destruct c;
+      unfold regs_erasure, reg_erasure, Pregmap.get in *;
+      repeat match goal with
+             | [|- match (?Rs ?R) with _ => _ end = _] =>
+               pose proof (Hrs R);
+                 destruct (Rs R);
+                 match goal with
+                 | [H: val_erasure _ _ |- _] =>
+                   inv H
+                 end
+             end; auto; try by exfalso.
+  Qed.
 
-  (* TODO: move this to the right place*)
-  Lemma get_erased_reg:
+  Import TraceErasure.
+
+  Lemma eval_addrmode_erase:
+    forall g a rs rs',
+      regs_erasure rs rs' ->
+      isPointer (eval_addrmode g a rs) -> 
+      eval_addrmode g a rs = eval_addrmode g a rs'.
+  Proof.
+    intros. unfold isPointer in *.
+    destruct (eval_addrmode g a rs) eqn:?; try by exfalso.
+    symmetry.
+    unfold eval_addrmode in *.
+    repeat match goal with
+           | [|-context[match ?Expr with _ => _ end]] =>
+             destruct Expr
+           end;
+      eauto with val_erasure regs_erasure.
+    eapply val_erasure_add_result with
+    (v1 := rs i0) (v2 := Val.add (Val.mul (rs i1) (Vint i2)) (Vint i3));
+      eauto with val_erasure regs_erasure.
+    eapply val_erasure_add_result with
+    (v2 := Val.add (Val.mul (rs i1) (Vint i2)) (Genv.symbol_address g i3 i4));
+      eauto with val_erasure regs_erasure.
+  Qed.
+
+  Lemma undef_regs_comm:
+    forall regs rs r,
+      undef_regs regs (rs # r <- Vundef) =
+      (undef_regs regs rs) # r <- Vundef.
+  Proof. Admitted. (*already proved*)
+
+  Lemma regs_erasure_undef:
+    forall regs rs rs',
+      regs_erasure rs rs' ->
+      regs_erasure (undef_regs regs rs) (undef_regs regs rs').
+  Proof.
+    induction regs; intros; simpl.
+    auto.
+    do 2 rewrite undef_regs_comm.
+    eapply regs_erasure_set.
+    eauto.
+    simpl; auto.
+  Qed.
+
+  Lemma regs_erasure_set_undef:
+    forall rs rs' r,
+      regs_erasure rs rs' ->
+      regs_erasure rs # r <- Vundef rs'.
+  Proof.
+    intros.
+    unfold regs_erasure, reg_erasure in *.
+    intros r'.
+    rewrite Pregmap.gsspec.
+    destruct (Pregmap.elt_eq r' r); subst;
+    simpl; auto.
+  Qed.
+  Hint Resolve regs_erasure_set_undef : regs_erasure.
+
+  
+  Lemma val_erasure_addrmode:
+    forall g (a : addrmode) rs rs'
+      (Hrs: regs_erasure rs rs'),
+      val_erasure (eval_addrmode g a rs) (eval_addrmode g a rs').
+  Proof with eauto 10 with val_erasure regs_erasure.
+    intros.
+    unfold eval_addrmode.
+    destruct a, base, ofs, const;
+      try destruct p; try destruct p0;
+      try match goal with
+          | [|- context[match ?Expr with _ => _ end]] =>
+            destruct Expr
+          end...
+  Qed.
+
+  Lemma compare_ints_erasure:
+    forall v1 v2 v1' v2' rs rs' m m'
+      (Hval_erasure: val_erasure v1 v1')
+      (Hval_erasure': val_erasure v2 v2')
+      (Hrs: regs_erasure rs rs')
+      (Hmem: mem_erasure m m'),
+      regs_erasure (compare_ints v1 v2 rs m)
+                   (compare_ints v1' v2' rs' m').
+  Proof with eauto 12 using val_erasure_cmpu with regs_erasure val_erasure.
+    intros.
+    unfold compare_ints...
+  Qed.
+
+  Hint Extern 0 (val_erasure Vundef _) => reflexivity : val_erasure.
+
+  Lemma compare_floats_erasure:
+    forall v1 v2 v1' v2' rs rs'
+      (Hval_erasure: val_erasure v1 v1')
+      (Hval_erasure2: val_erasure v2 v2')
+      (Hrs: regs_erasure rs rs'),
+      regs_erasure (compare_floats v1 v2 rs)
+                   (compare_floats v1' v2' rs').
+  Proof with eauto 10 using val_erasure_cmpu with regs_erasure val_erasure.
+    intros.
+    unfold compare_floats.
+    destruct v1,v2; inv Hval_erasure; inv Hval_erasure2; simpl;
+    eauto 6 with regs_erasure val_erasure;
+    try destruct v1'; try destruct v2';
+    eauto 6 with regs_erasure val_erasure;
+    unfold Val.of_bool;
+    repeat rewrite if_negb;
+    repeat match goal with
+           | [|- context[match ?Expr with | _ => _ end]] =>
+             destruct Expr eqn:?
+           end...
+  Qed.
+
+  Lemma compare_floats32_erasure:
+    forall v1 v2 v1' v2' rs rs'
+      (Hval_erasure: val_erasure v1 v1')
+      (Hval_erasure2: val_erasure v2 v2')
+      (Hrs: regs_erasure rs rs'),
+      regs_erasure (compare_floats32 v1 v2 rs)
+                   (compare_floats32 v1' v2' rs').
+  Proof with eauto 10 using val_erasure_cmpu with regs_erasure val_erasure.
+    intros.
+    unfold compare_floats32.
+    destruct v1,v2; inv Hval_erasure; inv Hval_erasure2; simpl;
+    eauto 6 with regs_erasure val_erasure;
+    try destruct v1'; try destruct v2';
+    eauto 6 with regs_erasure val_erasure;
+    unfold Val.of_bool;
+    repeat rewrite if_negb;
+    repeat match goal with
+           | [|- context[match ?Expr with | _ => _ end]] =>
+             destruct Expr eqn:?
+           end...
+  Qed.
+  
+  
+  Hint Resolve compare_ints_erasure compare_floats_erasure
+       compare_floats32_erasure val_erasure_addrmode
+       regs_erasure_undef : regs_erasure.
+  Hint Extern 0 (val_erasure (undef_regs _ _ # _ <- _ _) _) =>
+  eapply regs_erasure_set : regs_erasure.
+
+  Hint Transparent undef_regs: regs_erasure.
+
+    (* TODO: move this to the right place*)
+  Lemma get_reg_erasure:
     forall rs rs' r
-      (Herased_regs: erased_regs rs rs')
+      (Hregs_erasure: regs_erasure rs rs')
       (Hundef: rs r <> Vundef),
       rs r = rs' r.
   Proof.
     intros.
-    unfold erased_regs, erased_reg, Pregmap.get, erased_val in *.
-    specialize (Herased_regs r).
+    unfold regs_erasure, reg_erasure, Pregmap.get, val_erasure in *.
+    specialize (Hregs_erasure r).
     destruct (rs r); tauto.
   Qed.
 
-  Lemma mem_erasure_idempotent:
+  Lemma erasure_eval_testcond:
+    forall c rs rs' b,
+      regs_erasure rs rs' ->
+      eval_testcond c rs = Some b ->
+      eval_testcond c rs' = Some b.
+  Proof.
+    intros.
+    unfold eval_testcond in *.
+    destruct c;
+    repeat  match goal with
+      | [H: match ?Expr with | _ => _ end = _ |- _] =>
+        destruct Expr eqn:?
+      end; try discriminate;
+    repeat  match goal with
+            |[H: rs ?R = _ |- _] =>
+             erewrite get_reg_erasure  in H by (eauto; congruence);
+               rewrite H
+            |[H: Some _ = Some _ |- _] =>
+             inv H
+            end; auto.
+  Qed.
+
+
+  Parameter mem_erasure' : mem -> mem -> Prop.
+  Axiom mem_erasure'_erase:
     forall m m',
-      erasedMem m m' ->
-      erasedMem m (erasePerm m').
+      mem_erasure' m m' ->
+      mem_erasure m (erasePerm m').
+  
+  Lemma alloc_erasure':
+    forall m m' sz m2 m2' b b'
+      (Herased: mem_erasure m m')
+      (Halloc: Mem.alloc m 0 sz = (m2, b))
+      (Halloc': Mem.alloc m' 0 sz = (m2', b')),
+      mem_erasure' m2 m2' /\ b = b'.
   Proof.
   Admitted.
 
+  Lemma mem_free_erasure':
+    forall m m' sz m2 b
+      (Herased: mem_erasure m m')
+      (Hfree: Mem.free m b 0 sz = Some m2),
+    exists m2',
+      Mem.free m' b 0 sz = Some m2' /\
+      mem_erasure' m2 m2'.
+  Admitted.
+
+  Lemma mem_store_erased':
+    forall chunk m m' b ofs v v' m2
+      (Hstore: Mem.store chunk m b ofs v = Some m2)
+      (Herased: mem_erasure' m m')
+      (Hval_erasure: val_erasure v v') ,
+    exists m2', Mem.store chunk m' b ofs v' = Some m2'
+           /\ mem_erasure' m2 m2'.
+  Admitted.
+
+ Lemma mem_loadv_erased' :
+    forall (chunk : memory_chunk) (m m' : mem) (vptr v : val),
+      Mem.loadv chunk m vptr = Some v ->
+      mem_erasure' m m' ->
+      exists v' : val, Mem.loadv chunk m' vptr = Some v' /\ val_erasure v v'.
+  
+  Axiom mem_erasure_erasure':
+    forall m m',
+      mem_erasure m m' ->
+      mem_erasure' m m'.
+  
+  Lemma exec_instr_erased:
+    forall (g : genv) (fn : function) (i : instruction) (rs rs' rs2: regset)
+      (m m' m2 : mem) ev
+      (HeraseCores: regs_erasure rs rs')
+      (HerasedMem: mem_erasure m m')
+      (Hexec_ev: Asm_event.drf_instr g (fn_code fn) i rs m = Some ev)
+      (Hexec: exec_instr g fn i rs m = Next rs2 m2),
+    exists rs2' m2' ev',
+      exec_instr g fn i rs' m' = Next rs2' m2' /\
+      Asm_event.drf_instr g (fn_code fn) i rs' m' = Some ev' /\
+      regs_erasure rs2 rs2' /\ mem_erasure m2 (erasePerm m2') /\
+      mem_event_list_erasure ev ev'.
+  Proof.
+    intros.
+    destruct i; simpl in *;
+    unfold goto_label in *;
+    repeat match goal with
+           | [H: context[match eval_testcond ?C rs with _ => _ end] |- _] =>
+             destruct (eval_testcond C rs) as [b|] eqn:?
+           | [H: eval_testcond ?C rs = Some _ |- _] =>
+             erewrite <- eval_testcond_erasure with (rs := rs)
+               by (eauto; rewrite H; congruence);
+               rewrite H;
+               destruct b
+           end;
+    (* see if this does anything*)
+      repeat match goal with
+             | [|- match (?Rs ?R) with _ => _ end = _] =>
+               pose proof (Hrs R);
+                 destruct (Rs R);
+                 match goal with
+                 | [H: val_erasure _ _ |- _] =>
+                   inv H
+                 end
+             end; auto;
+    repeat match goal with
+           | [H: match ?Expr with _ => _ end = _ |- _] =>
+             destruct Expr eqn:?
+           end; try discriminate;
+    try match goal with
+        | [H: Mem.alloc m 0 ?Sz = _ |- _] =>
+          destruct (Mem.alloc m' 0 Sz) as [? ?] eqn:Halloc';
+            eapply alloc_erasure' in Halloc'; eauto;
+            destruct Halloc'; subst
+        | [H: Mem.free _ _ _ _ = _ |- _] =>
+          eapply mem_free_erasure' in H; eauto;
+          destruct H as [? [? Herasure']];
+          eapply mem_erasure'_erase in Herasure'
+        end;
+    repeat match goal with
+           | [H: Mem.store ?Chunk ?M ?B ?Ofs (rs ?R) = _,
+                 H1: mem_erasure' ?M ?M2 |- _] =>
+             eapply mem_store_erased' with (m' := M2) (v' := rs' R) in H;
+               eauto with regs_erasure val_erasure;
+               destruct H as [? [? ?]]
+           | [H: Mem.loadv _ ?M (Vptr _ _) = _, H2: mem_erasure ?M _ |- _] =>
+             eapply mem_loadv_erased in H; eauto;
+             destruct H as [? [? ?]]
+           end;
+    try match goal with
+        | [H: exec_store ?G ?CHUNK ?M ?A ?RS ?RS0 _ = _ |- _] =>
+          unfold exec_store in *;
+            destruct (Mem.storev CHUNK M (eval_addrmode G A RS) (RS RS0)) eqn:?;
+                     inv H
+        | [H: exec_load ?G ?CHUNK ?M ?A ?RS ?RD = _ |- _] =>
+          unfold exec_load in *;
+            destruct (Mem.loadv CHUNK M (eval_addrmode G A RS)) eqn:?;
+                     inv H
+        | [H: Next _ _ = Next _ _ |- _] =>
+          inv H
+        end;    
+    try match goal with
+        | [H: Mem.loadv _ _ (eval_addrmode ?G ?A rs) = _ |- _] =>
+          pose proof (loadv_pointer _ _ _ H);
+            erewrite <- eval_addrmode_erase by (eauto);
+          eapply mem_loadv_erased with
+          (m' := m') (vptr := eval_addrmode G A rs) in H;
+            eauto with val_erasure regs_erasure;
+            destruct H as [? [? ?]]
+        | [H: Mem.storev _ _ (eval_addrmode ?G ?A rs) (rs ?R) = _ |- _] =>
+          pose proof (storev_pointer _ _ _ _ H);
+            erewrite <- eval_addrmode_erase by (eauto);
+            eapply mem_storev_erased with
+            (m' := m') (vptr := eval_addrmode G A rs) (v' := rs' R) in H;
+            eauto with val_erasure regs_erasure;
+            destruct H as [? [? ?]]
+        | [H: Val.divs _ _ = _, H2: Val.mods _ _ = _ |- _] =>
+          erewrite divs_ren with (v1' := rs' EAX) (v2' := rs' # EDX <- Vundef r1) in H;
+            eauto with reg_renamings val_renamings;
+            erewrite mods_ren with (v1' := rs' EAX) (v2' := rs' # EDX <- Vundef r1)
+              in H2; eauto with reg_renamings val_renamings
+        | [H: Val.divu _ _ = _, H2: Val.modu _ _ = _ |- _] =>
+          erewrite divu_ren with (v1' := rs' EAX) (v2' := rs' # EDX <- Vundef r1) in H;
+            eauto with reg_renamings val_renamings;
+            erewrite modu_ren with (v1' := rs' EAX) (v2' := rs' # EDX <- Vundef r1)
+              in H2; eauto with reg_renamings val_renamings
+        end;
+      repeat match goal with
+             | [H: Mem.loadbytes ?M _ _ _ = _, H2: mem_erasure ?M _ |- _] =>
+               eapply loadbytes_erasure in H; eauto;
+               destruct H as [? [? ?]]
+             end;
+    unfold nextinstr_nf, nextinstr, Vone, Vzero;
+    repeat match goal with
+           | [H: Val.divu (rs ?R) (rs # ?R2 <- ?V ?R3) = _ |- _] =>
+             eapply val_erasure_divu_result with (v1' := rs' R)
+                                                   (v2' := rs' # R2 <- V R3) in H;
+               eauto with regs_erasure val_erasure;
+               rewrite H
+           | [H: Val.modu (rs ?R) (rs # ?R2 <- ?V ?R3) = _ |- _] =>
+             eapply val_erasure_modu_result with (v1' := rs' R)
+                                                   (v2' := rs' # R2 <- V R3) in H;
+               eauto with regs_erasure val_erasure;
+               rewrite H
+           | [H: Val.divs (rs ?R) (rs # ?R2 <- ?V ?R3) = _ |- _] =>
+             eapply val_erasure_divs_result with (v1' := rs' R)
+                                                   (v2' := rs' # R2 <- V R3) in H;
+               eauto with regs_erasure val_erasure;
+               rewrite H
+           | [H: Val.mods (rs ?R) (rs # ?R2 <- ?V ?R3) = _ |- _] =>
+             eapply val_erasure_mods_result with (v1' := rs' R)
+                                                   (v2' := rs' # R2 <- V R3) in H;
+               eauto with regs_erasure val_erasure;
+               rewrite H
+           | [|- context[eval_testcond ?C rs']] =>
+             destruct (eval_testcond C rs') as [[]|] eqn:?
+           | [H: eval_addrmode _ _ _ = _, H2: Mem.loadv _ _ _ = _ |- _] =>
+             rewrite H in H2
+           | [H: eval_addrmode _ _ _ = _, H2: Mem.storev _ _ _ _ = _ |- _] =>
+             rewrite H in H2
+           | [H: eval_addrmode _ _ _ = _ |- context[eval_addrmode _ _ _]] =>
+             rewrite H
+           | [H: Mem.loadv _ _ _ = _ |- _] =>
+             rewrite H; clear H; eauto
+           | [H: Mem.storev _ _ _ _ = _ |- _] =>
+             rewrite H; clear H; eauto
+           | [H: Mem.loadbytes _ _ _ _ = _ |- _] =>
+             rewrite H; clear H
+           | [|- _ /\ _] => split; eauto
+           | [H: Some _ = Some _ |- _] =>
+             inv H
+           | [H: rs ?R = _ |- _ ] =>
+             erewrite get_reg_erasure in H by (eauto; congruence);
+               try rewrite H; clear H
+           | [H: ?Expr = _ |- context[?Expr]] =>
+             rewrite H; clear H
+           | [|- regs_erasure _ _] =>
+             eauto 20 with regs_erasure val_erasure
+           | [|- mem_erasure _ (erasePerm _)] =>
+             eauto using mem_erasure_idempotent
+           | [|- mem_event_list_erasure _ _] =>
+             constructor
+           | [|- mem_event_erasure _ _ ] => constructor
+           | [|- memval_erasure_list _ _] =>
+             eauto with val_erasure regs_erasure
+           | [|- exists _ _ _, _ ] => do 3 eexists; split; try reflexivity          
+           end; try (by exfalso); try assumption.
+    destruct (eval_testcond c rs) as [[]|] eqn:Heq; simpl;
+    try pose proof (erasure_eval_testcond _ HeraseCores Heq);
+    try congruence;
+    eauto 8 with regs_erasure val_erasure.
+    destruct (eval_testcond c rs) as [[]|] eqn:Heq; simpl;
+    try pose proof (erasure_eval_testcond _ HeraseCores Heq);
+    try congruence;
+    eauto 8 with regs_erasure val_erasure.
+    assert (Heval: eval_testcond c rs = None).
+    { destruct (eval_testcond c rs) eqn:Heval;
+      auto.
+      eapply erasure_eval_testcond in Heval; eauto;
+      congruence.
+    }
+    rewrite Heval. simpl.
+    eauto 8 with regs_erasure val_erasure.
+    eapply mem_erasure'_erase; eauto.
+  Qed.
+
+  Lemma extcall_arg_erasure:
+    forall m m' loc arg rs rs' ev
+      (Harg: extcall_arg rs m loc arg)
+      (Harg_ev: Asm_event.extcall_arg_ev rs m loc arg ev)
+      (Hmem_obs_eq: mem_erasure m m') 
+      (Hrs : regs_erasure rs rs'),
+    exists arg' ev',
+      Asm_event.extcall_arg_ev rs' m' loc arg' ev' /\
+      extcall_arg rs' m' loc arg' /\
+      val_erasure arg arg' /\
+      mem_event_list_erasure ev ev'.
+  Proof with eauto with val_erasure regs_erasure.
+    intros.
+    inversion Harg; subst.
+    - inversion Harg_ev; subst.
+      exists (rs' (preg_of r)), [::];
+      (repeat split); try econstructor...
+    - inversion Harg_ev; subst.
+      eapply mem_loadv_erased in H0; eauto.
+      destruct H0 as [arg' [Hload' Harg_erasure]].
+      eapply loadbytes_erasure in H6; eauto.
+      destruct H6 as [bytes' [Hloadbytes' Hbytes_erasure]].
+      rewrite H3 in Hload'. simpl in Hload'.
+      assert (Val.add (rs' ESP) (Vint (Int.repr (Stacklayout.fe_ofs_arg + 4 * ofs)))
+              = Vptr b z)
+        by (eapply val_erasure_add_result; eauto with val_erasure regs_erasure ).
+        exists arg', [:: Read b (Int.unsigned z) (size_chunk (chunk_of_type ty))
+                  bytes'].
+      (repeat split); try econstructor...
+      eapply Mem.loadbytes_load in Hloadbytes'; eauto.
+      rewrite Hloadbytes' in Hload'. inv Hload'.
+      reflexivity.
+      rewrite H. simpl; auto.
+      econstructor; eauto.
+      constructor.
+  Qed.
+      
   Lemma extcall_arguments_erasure:
     forall m m' ef args rs rs' ev
       (Hexternal: extcall_arguments rs m (ef_sig ef) args)
       (Hexternal_ev: Asm_event.extcall_arguments_ev rs m (ef_sig ef) args ev)
-      (Hmem_obs_eq: erasedMem m m') 
-      (Hrs : erased_regs rs rs'),
-    exists args',
-      Asm_event.extcall_arguments_ev rs' m' (ef_sig ef) args' ev /\
+      (Hmem_obs_eq: mem_erasure m m') 
+      (Hrs : regs_erasure rs rs'),
+    exists args' ev',
+      Asm_event.extcall_arguments_ev rs' m' (ef_sig ef) args' ev' /\
       extcall_arguments rs' m' (ef_sig ef) args' /\
-      erased_val_list args args'.
+      val_erasure_list args args' /\
+      mem_event_list_erasure ev ev'.
   Proof.
-  Admitted.
+    intros.
+    unfold extcall_arguments, Asm_event.extcall_arguments_ev in *.
+    generalize dependent ev.
+    generalize dependent (Conventions1.loc_arguments (ef_sig ef)).
+    induction args; intros.
+    - inversion Hexternal; subst.
+      inv Hexternal_ev.
+      exists [::], [::].
+      repeat split;
+        constructor.
+    - inversion Hexternal; subst.
+      inv Hexternal_ev.
+      destruct (IHargs _ H3 _ H9) as (args' & T2' & Hargs_ev &
+                                      Hls & Hargs_erasure & HT_erasure2).
+      eapply extcall_arg_erasure in H2; eauto.
+      destruct H2 as (arg' & T1' & Harg_ev' & Harg' & Harg_erasure' & HT_erasure1).
+      exists (arg' :: args'), (T1' ++ T2').
+      repeat split; try econstructor; eauto.
+      eapply mem_event_list_erasure_cat; eauto.
+  Qed.
+      
+
+  
+  Lemma load_frame_store_nextblock:
+    forall m m2 stk args tys
+      (Hload_frame: load_frame.store_args m stk args tys = Some m2),
+      Mem.nextblock m2 = Mem.nextblock m.
+  Proof.
+  Admitted. (*already done*)
+
+  Lemma load_frame_store_args_rec_erasure:
+    forall m m2 m' args args' T tys stk ofs
+      (Hmem: mem_erasure m m')
+      (Hargs: val_erasure_list args args')
+      (Hload_frame: load_frame.store_args_rec m stk ofs args tys = Some m2)
+      (Hargs_ev: Asm_event.store_args_ev_rec stk ofs args tys = Some T),
+    exists m2' T',
+      load_frame.store_args_rec m' stk ofs args' tys = Some m2' /\
+      Asm_event.store_args_ev_rec stk ofs args' tys = Some T' /\
+      mem_erasure m2 m2' /\
+      mem_event_list_erasure T T'.
+  Proof with eauto with val_renamings reg_renamings.
+    intros.
+    generalize dependent tys.
+    generalize dependent args'.
+    generalize dependent ofs.
+    generalize dependent m'.
+    generalize dependent m.
+    generalize dependent T.
+    induction args; intros.
+    - unfold load_frame.store_args_rec, Asm_event.store_args_ev_rec in *.
+      simpl in *. destruct tys; intros; try discriminate.
+      inv Hargs; inv Hload_frame; inv Hargs_ev.
+      simpl. do 2 eexists.
+      split; eauto. split; eauto. split; eauto.
+      constructor.
+    - simpl in *.
+      inv Hargs.
+      destruct tys; simpl in *; try discriminate;
+      destruct t;
+      repeat match goal with
+      | [H: match ?Expr with _ => _ end = _ |- _] =>
+        destruct Expr eqn:?
+      end; try discriminate; subst;
+      unfold load_frame.store_stack in *;
+      inv Hargs_ev;
+      try match goal with
+          | [H: val_erasure (Vlong _) _ |- _] =>
+            inv H
+          end;
+      try (eapply mem_storev_erased in Heqo0; eauto;
+           destruct Heqo0 as [m2' [Hstorev' Hmem_erased']];
+           rewrite Hstorev'); simpl;
+      try destruct (IHargs _ _ _ Hmem_erased' _ _ H3 _ Hload_frame Heqo)
+        as (m2'' & T'' & Hstore_args'' & Hstore_args_ev'' & Hmem_erased'' &
+            Hevent_erasure'');
+        try match goal with
+             | [|- context[encode_val ?Chunk _]] =>
+               exists m2'', (Write stk
+                              (Int.unsigned
+                                 (Int.repr
+                                    match ofs with
+                                    | 0 => 0
+                                    | Z.pos y' => Z.pos y'~0~0
+                                    | Z.neg y' => Z.neg y'~0~0
+                                    end)) (encode_val Chunk v') :: T'')
+                         end;
+      repeat match goal with
+             | [H: ?Expr = _ |- context[?Expr]] =>
+               rewrite H
+             end;
+      try (split; auto; split; auto;
+           split; auto; constructor);
+      try constructor; eauto using encode_val_erasure.
+      eapply mem_storev_erased in Heqo0; simpl; eauto.
+      destruct Heqo0 as [m0' [Hstorev' Hmem_erased']]; simpl in Hstorev'.
+      rewrite Hstorev'.
+      eapply mem_storev_erased in Heqo1; simpl; eauto.
+      destruct Heqo1 as [m1' [Hstorev1' Hmem_erased1']]; simpl in Hstorev1'.
+      rewrite Hstorev1'.
+      destruct (IHargs _ _ _ Hmem_erased1' _ _ H3 _ Hload_frame Heqo)
+        as (m2'' & T'' & Hstore_args'' & Hstore_args_ev'' & Hmem_erased'' &
+            Hevent_erasure'').
+      exists m2'', [:: Write stk
+                 (Int.unsigned
+                    (Int.repr
+                       match ofs + 1 with
+                       | 0 => 0
+                       | Z.pos y' => Z.pos y'~0~0
+                       | Z.neg y' => Z.neg y'~0~0
+                       end))
+                 (inj_bytes (encode_int 4 (Int.unsigned (Int64.hiword i)))),
+               Write stk
+                 (Int.unsigned
+                    (Int.repr
+                       match ofs with
+                       | 0 => 0
+                       | Z.pos y' => Z.pos y'~0~0
+                       | Z.neg y' => Z.neg y'~0~0
+                       end))
+                 (inj_bytes (encode_int 4 (Int.unsigned (Int64.loword i))))
+               & T''].
+      split; auto.
+      rewrite Hstore_args_ev''.
+      split; auto. split; auto.
+      do 2 constructor.
+      apply inj_bytes_erasure.
+      constructor.
+      apply inj_bytes_erasure.
+      auto.
+  Qed.
+  
+  Lemma load_frame_store_args_erasure:
+    forall m m2 m' args args' T tys stk
+      (Hmem: mem_erasure m m')
+      (Hargs: val_erasure_list args args')
+      (Hload_frame: load_frame.store_args m stk args tys = Some m2)
+      (Hargs_ev: Asm_event.store_args_events stk args tys = Some T),
+    exists m2' T',
+      load_frame.store_args m' stk args' tys = Some m2' /\
+      Asm_event.store_args_events stk args' tys = Some T' /\
+      mem_erasure m2 m2' /\
+      mem_event_list_erasure T T'.
+  Proof.
+    intros.
+    unfold load_frame.store_args in *.
+    eapply load_frame_store_args_rec_erasure; eauto.
+  Qed.
 
   Lemma evstep_erase:
     forall ge c1 c1' c2 ev m1 m1' m2
-      (HeraseCores: erasedCores c1 c1')
-      (HerasedMem: erasedMem m1 m1')
+      (HeraseCores: core_erasure c1 c1')
+      (HerasedMem: mem_erasure m1 m1')
       (Hstep: ev_step Sem ge c1 m1 ev c2 m2),
-    exists c2' m2',
-      ev_step Sem ge c1' m1' ev c2' m2' /\
-      erasedCores c2 c2' /\ erasedMem m2 (erasePerm m2').
-  Proof with eauto with erased.
+    exists c2' m2' ev',
+      ev_step Sem ge c1' m1' ev' c2' m2' /\
+      core_erasure c2 c2' /\ mem_erasure m2 (erasePerm m2') /\
+      mem_event_list_erasure ev ev'.
+  Proof with eauto with erased trace_erasure.
     intros.
     destruct c1 as [rs1 loader1 | |]; simpl in *;
     destruct c1' as [rs1' loader1' | |]; try by exfalso.
     - destruct HeraseCores as [Hrs Hloader].
-      unfold erased_loader in Hloader; subst.
+      unfold loader_erasure in Hloader; subst.
       inversion Hstep; subst; try (by exfalso).
       + assert (Hpc' : rs1' PC = Vptr b ofs)
-          by (erewrite get_erased_reg in H1; eauto;
+          by (erewrite get_reg_erasure in H1; eauto;
               rewrite H1; discriminate).
-      destruct (exec_instr_erased _ _ _ Hrs HerasedMem H4)
-        as (rs2' & m2' & Hexec' & Hrs2 & Hm2).
-      exists (State rs2' loader1'), m2'.
+      destruct (exec_instr_erased _ _ _ Hrs HerasedMem H9 H4)
+        as (rs2' & m2' & ev' & Hexec' & Hexec_ev' & Hrs2 & Hm2 & Hev_erasure).
+      exists (State rs2' loader1'), m2', ev'.
       repeat match goal with
              | [ |- _ /\ _] =>
                split; simpl; eauto with erased
              end.
       econstructor...
-      admit.
     + assert (Hpc' : rs1' PC = Vptr b Int.zero)
-          by (erewrite get_erased_reg in H1; eauto;
+          by (erewrite get_reg_erasure in H1; eauto;
               rewrite H1; discriminate).
       assert (Hargs' := extcall_arguments_erasure _ H3 H8 HerasedMem Hrs).
-      destruct Hargs' as (args' & Hargs_ev' & Hargs' & Hargs_erasure).
-      exists (Asm_CallstateOut ef args' rs1' loader1'), m1'.
+      destruct Hargs' as (args' & ev' & Hargs_ev' & Hargs'
+                          & Hargs_erasure & Hev_erasure).
+      exists (Asm_CallstateOut ef args' rs1' loader1'), m1', ev'.
       split. econstructor...
-      split. simpl; repeat split...
-      eapply mem_erasure_idempotent; eauto.
+      split; first by eauto.
+      split; first by (eapply mem_erasure_idempotent; eauto).
+      auto.
     - destruct HeraseCores as (? & Herased_args & ? & ?).
       subst.
       inversion Hstep; subst.
       destruct (Mem.alloc m1' 0 (4*z)) as [m2' stk'] eqn:Halloc'.
-
-      Lemma alloc_erasure:
-        forall m m' sz m2 m2' b b'
-          (Herased: erasedMem m m')
-          (Halloc: Mem.alloc m 0 sz = (m2, b))
-          (Halloc': Mem.alloc m' 0 sz = (m2', b')),
-          erasedMem m2 m2' /\ b = b'.
-      Admitted.
       destruct (alloc_erasure HerasedMem H8 Halloc') as (HerasedMem2 & ?).
-      subst.      
-      assert (erased_regs
+      subst stk'.
+      assert (regs_erasure
                 ((((Pregmap.init Vundef) # PC <- (Vptr f0 Int.zero)) # RA <- Vzero)
-                   # ESP <- (Vptr stk' Int.zero))
+                   # ESP <- (Vptr stk Int.zero))
                 ((((Pregmap.init Vundef) # PC <- (Vptr f0 Int.zero)) # RA <- Vzero)
-                   # ESP <- (Vptr stk' Int.zero)))
-        by (eapply erased_regs_refl).
+                   # ESP <- (Vptr stk Int.zero)))
+        by (eapply regs_erasure_refl).
       assert (load_frame.args_len_rec args0 tys0 = Some z).
       { clear - Herased_args H3.
         generalize dependent tys0.
@@ -341,55 +919,20 @@ Module X86CoreErasure <: CoreErasure X86SEM.
         destruct a; inv H1; try discriminate;
         auto.
       }
-
-      Lemma load_frame_store_nextblock:
-        forall m m2 stk args tys
-          (Hload_frame: load_frame.store_args m stk args tys = Some m2),
-          Mem.nextblock m2 = Mem.nextblock m.
-      Proof.
-      Admitted. (*already done*)
-
-      Lemma load_frame_store_args_erasure:
-        forall m m2 m' args args' T tys
-          (Hmem: erasedMem m m')
-          (Hargs: erased_val_list args args')
-          (Hload_frame: load_frame.store_args m stk args tys = Some m2)
-          (Hargs_ev: Asm_event.store_args_events stk args tys0 = Some T),
-        exists m2',
-          load_frame.store_args m' stk args' tys = Some m2' /\
-          load_frame.store_args stk args' tys = Some T /\
-          erasedMem m2 m'.
-      Proof.
-      Admitted.
-
-        Lemma extcall_arguments_erasure:
-    forall m m' ef args rs rs' ev
-      (Hexternal: extcall_arguments rs m (ef_sig ef) args)
-      (Hexternal_ev: Asm_event.extcall_arguments_ev rs m (ef_sig ef) args ev)
-      (Hmem_obs_eq: erasedMem m m') 
-      (Hrs : erased_regs rs rs'),
-    exists args',
-      Asm_event.extcall_arguments_ev rs' m' (ef_sig ef) args' ev /\
-      extcall_arguments rs' m' (ef_sig ef) args' /\
-      erased_val_list args args'.
-  Proof.
-  Admitted.
-      
-      assert (Hnb := load_frame_store_nextblock _ _ _ _ H9).
       eapply load_frame_store_args_erasure in H9; eauto.
-      destruct H8 as [m2' [Hload_frame' Hobs_eq']].
-      assert (Hnb' := load_frame_store_nextblock _ _ _ _ Hload_frame').
-
-      exists (State ((((Pregmap.init Vundef) # PC <- (Vptr f1 Int.zero)) # RA <- Vzero)
-                  # ESP <- (Vptr stk' Int.zero)) (mk_load_frame stk' retty0)), m2', f'.
-      unfold Mem.valid_block in *.
-      rewrite Hnb Hnb'.
-      repeat match goal with
-             | [ |- _ /\ _] =>
-               split; simpl; eauto
-             end.
+      destruct H9 as [m2'' [T' [Hstore_args' [Hstore_args_ev'
+                                               [HerasedMem' HerasedT]]]]].
+      exists (State ((((Pregmap.init Vundef) # PC <- (Vptr f0 Int.zero)) # RA <- Vzero)
+                  # ESP <- (Vptr stk Int.zero)) (mk_load_frame stk retty0)), m2'',
+      (Alloc stk 0 (4 * z) :: T').
+      split.
       econstructor; eauto.
-  - inversion Hcorestep; by exfalso.
+      econstructor...
+      split.
+      eapply mem_erasure_idempotent; eauto.
+      econstructor; eauto.
+      econstructor; eauto.
+  - inversion Hstep; by exfalso.
   Qed.
 
 End X86CoreErasure.
